templates/lockfree/skiplist.v
@@ -12,16 +12,71 @@ From iris.bi.lib Require Import fractional.
 Set Default Proof Using "All".
 From iris.bi.lib Require Import fractional.
 From flows Require Export multiset_flows keyset_ra2 bool_ra.
-From flows Require Export hindsight node_module.
+From flows Require Export hindsight traverse_module.
 
-Module SKIPLIST (NODE : NODE_IMPL) <: DATA_STRUCTURE.
-  Export NODE.
+Module SKIPLIST (TR : TRAVERSE) <: DATA_STRUCTURE.
+  Export TR.NODE TR.
   
-  Parameter L : nat. (* Maxlevels *)
+  (* Parameter L : nat. (* Maxlevels *) *)
   Parameter W : nat. (* Keyspace *)
 
   (* Template Algorithms *)
+(*
+  Definition traverse_i : heap_lang.val :=
+    rec: "tri" "i" "pred" "predn" "curr" "k" :=
+      let: "fn_curr" := findNext "curr" "i" in
+      let: "m" := Fst "fn_curr" in
+      let: "succ" := Snd "fn_curr" in
+      if: "m" then
+        "tri" "i" "pred" "predn" "succ" "k"
+      else
+        let: "res" := compareKey "curr" "k" in
+          if: "res" = #0 then 
+          "tri" "i" "curr" "succ" "succ" "k"
+          else
+            match: changeNext "pred" "predn" "curr" "i" with
+              NONE => NONE
+            | SOME "_" => 
+              if: "res" = #1 then
+                SOME ("pred", "curr", #true)
+              else
+                SOME ("pred", "curr", #false).
 
+  Definition traverse_pop : heap_lang.val :=
+    λ: "k" "preds" "succs" "i",
+      let: "pred" := ! ("preds" +ₗ ("i" + #1)) in
+      let: "fn_pred" := findNext "pred" "i" in
+      let: "curr" := Snd "fn_pred" in
+      let: "ores" := traverse_i "i" "pred" "pred" "curr" "k" in
+      match: "ores" with
+        NONE => NONE
+      | SOME "pred_succ_res" =>
+        let: "pred" := Fst (Fst "pred_succ_res") in
+        let: "succ" := Snd (Fst "pred_succ_res") in
+        let: "res" := Snd "pred_succ_res" in
+        "preds" +ₗ "i" <- "pred";;
+        "succs" +ₗ "i" <- "succ";;
+        SOME ("preds", "succs", "res") end.
+
+  Definition traverse_rec : heap_lang.val :=
+    rec: "trec" "k" "preds" "succs" "i" :=
+      let: "ores" := traverse_pop "k" "preds" "succs" "i" in
+      match: "ores" with 
+        NONE => "trec" "k" "preds" "succs" #(L-2)%nat
+      | SOME "res" => 
+        if: "i" = #0 then
+          "res"
+        else
+          "trec" "k" "preds" "succs" ("i" - #1) end.
+  
+  Definition traverse : heap_lang.val :=
+    λ: "h" "t" "k",
+      let: "preds" := AllocN #L "h" in
+      let: "succs" := AllocN #L "t" in
+      traverse_rec "k" "preds" "succs" #(L-2)%nat.  
+*)
+
+(*
   Definition traverse_i : heap_lang.val :=
     rec: "tri" "i" "pred" "curr" "k" :=
       let: "fn_curr" := findNext "curr" "i" in
@@ -73,6 +128,7 @@ Module SKIPLIST (NODE : NODE_IMPL) <: DATA_STRUCTURE.
       let: "preds" := AllocN #L "h" in
       let: "succs" := AllocN #L "t" in
       traverse_rec "k" "preds" "succs" #(L-2)%nat.  
+*)
 
   Definition search : heap_lang.val :=
     λ: "h" "t" "k",
