templates/lockfree/harris.v
@@ -1,0 +1,1564 @@
+From iris.algebra Require Import excl auth cmra gmap agree gset numbers.
+From iris.algebra.lib Require Import dfrac_agree.
+From iris.heap_lang Require Export notation locations lang.
+From iris.base_logic.lib Require Export invariants.
+From iris.program_logic Require Export atomic.
+From iris.proofmode Require Import tactics.
+From iris.heap_lang Require Import proofmode par.
+From iris.bi.lib Require Import fractional.
+Set Default Proof Using "All".
+From iris.bi.lib Require Import fractional.
+Require Import list_flow_upd_unlink.
+From flows Require Import array_util node_module.
+From flows Require Import traverse_module traverse_spec_module skiplist_util.
+
+Module HARRIS <: TRAVERSE.
+  Declare Module NODE : NODE_IMPL.
+  
+  Definition traverse_i : heap_lang.val :=
+    rec: "tri" "i" "pred" "predn" "curr" "k" :=
+      let: "fn_curr" := findNext "curr" "i" in
+      let: "m" := Fst "fn_curr" in
+      let: "succ" := Snd "fn_curr" in
+      if: "m" then
+        "tri" "i" "pred" "predn" "succ" "k"
+      else
+        let: "res" := compareKey "curr" "k" in
+        if: "res" = #0 then 
+          "tri" "i" "curr" "succ" "succ" "k"
+        else
+          if: "predn" = "curr" then
+            if: "res" = #1 then
+              SOME ("pred", "curr", #true)
+            else
+              SOME ("pred", "curr", #false)
+          else
+            match: changeNext "pred" "predn" "curr" "i" with
+              NONE => NONE
+            | SOME "_" => 
+              let: "fn_curr" := findNext "curr" "i" in
+              let: "m'" := Fst "fn_curr" in
+              if: "m'" then
+                NONE
+              else
+                if: "res" = #1 then
+                  SOME ("pred", "curr", #true)
+                else
+                  SOME ("pred", "curr", #false) end.
+
+  Definition traverse_pop : heap_lang.val :=
+    λ: "k" "preds" "succs" "i",
+      let: "pred" := ! ("preds" +ₗ ("i" + #1)) in
+      let: "fn_pred" := findNext "pred" "i" in
+      let: "curr" := Snd "fn_pred" in
+      let: "ores" := traverse_i "i" "pred" "curr" "curr" "k" in
+      match: "ores" with
+        NONE => NONE
+      | SOME "pred_succ_res" =>
+        let: "pred" := Fst (Fst "pred_succ_res") in
+        let: "succ" := Snd (Fst "pred_succ_res") in
+        let: "res" := Snd "pred_succ_res" in
+        "preds" +ₗ "i" <- "pred";;
+        "succs" +ₗ "i" <- "succ";;
+        SOME ("preds", "succs", "res") end.
+
+  Definition traverse_rec : heap_lang.val :=
+    rec: "trec" "k" "preds" "succs" "i" :=
+      let: "ores" := traverse_pop "k" "preds" "succs" "i" in
+      match: "ores" with 
+        NONE => "trec" "k" "preds" "succs" #(L-2)%nat
+      | SOME "res" => 
+        if: "i" = #0 then
+          "res"
+        else
+          "trec" "k" "preds" "succs" ("i" - #1) end.
+  
+  Definition traverse : heap_lang.val :=
+    λ: "h" "t" "k",
+      let: "preds" := AllocN #L "h" in
+      let: "succs" := AllocN #L "t" in
+      traverse_rec "k" "preds" "succs" #(L-2)%nat.  
+
+End HARRIS.
+
+Module HARRIS_SPEC <: TRAVERSE_SPEC.
+  Module TR := HARRIS.
+  Import HARRIS.
+
+  Definition traversal_inv Σ Hg1 Hg2 Hg3 γ_m t0 i k p c : iProp Σ :=
+    (∃ s, past_state Σ Hg1 Hg2 Hg3 γ_m t0 s ∗ ⌜p ∈ FP s ∧ Key s p < k ∧ 
+      Marki s p 0 = false ∧ i < Height s p ∧ (i = 0 → Nexti s p i = Some c)⌝)
+  ∗ (∃ s, past_state Σ Hg1 Hg2 Hg3 γ_m t0 s ∗ ⌜c ∈ FP s ∧ i < Height s c⌝).
+
+  Lemma traversal_inv_hd_tl Σ Hg1 Hg2 Hg3 γ_m γ_t γ_mt hd tl M T s tid t0 k:
+    ⌜M !!! T ≡ s⌝ -∗ 
+    ⌜per_tick_inv hd tl s⌝ -∗
+    ⌜1 < L⌝ -∗
+    ⌜0 < k < W⌝ -∗
+    thread_start Σ Hg1 Hg2 Hg3 γ_t γ_mt tid t0 -∗
+    hist Σ Hg1 Hg2 Hg3 γ_t γ_m M T -∗
+      |==> traversal_inv Σ Hg1 Hg2 Hg3 γ_m t0 (L-1) k hd tl ∗ hist Σ Hg1 Hg2 Hg3 γ_t γ_m M T.
+  Proof.
+    iIntros "%Habs %PT %HL %Range_k #Thd_st Hist".
+    iPoseProof (snapshot_current with "[%] [#] [$]") 
+      as ">(#Past_s&Hist)"; try done.
+    destruct PT as ((H1'&H2'&H3'&H4'&H5'&H6'&H7'&H8'&H9')&_).
+    iModIntro. iFrame. iSplit; iExists s; iFrame "Past_s".
+    - iPureIntro; repeat split; try (done || lia).
+      set_solver. apply H4'. lia.
+    - iPureIntro; repeat split; try (done || lia). set_solver.
+  Qed. 
+
+  Definition past_marked_segment Σ Hg1 Hg2 Hg3 γ_m t0 i pn ls c : iProp Σ :=
+    match ls with 
+    | [] => (∃ s, past_state Σ Hg1 Hg2 Hg3 γ_m t0 s ∗ 
+      ⌜pn ∈ FP s ∧ Marki s pn i = true ∧ Nexti s pn i = Some c⌝)
+    | n :: _ => 
+    (∃ s, past_state Σ Hg1 Hg2 Hg3 γ_m t0 s ∗ 
+      ⌜pn ∈ FP s ∧ Marki s pn i = true ∧ Nexti s pn i = Some n⌝)
+    ∗ (∀ j, ⌜j < length ls - 1⌝ -∗ 
+        (∃ s, past_state Σ Hg1 Hg2 Hg3 γ_m t0 s 
+          ∗ ⌜(ls !!! j) ∈ FP s ∧ Marki s (ls !!! j) i = true 
+              ∧ Nexti s (ls !!! j) i = Some (ls !!! ((j+1)%nat))⌝))
+    ∗ (let last := ls !!! (length ls - 1) in
+        ∃ s, past_state Σ Hg1 Hg2 Hg3 γ_m t0 s 
+        ∗ ⌜last ∈ FP s ∧ Marki s last i = true 
+            ∧ Nexti s last i = Some c⌝) end.
+
+  
+  Lemma traverse_i_spec Σ Hg1 Hg2 Hg3 ls N γ_t γ_r γ_m γ_mt γ_msy r tid t0 k 
+    (i: nat) (p pn c: Node):
+    main_inv Σ Hg1 Hg2 Hg3 N γ_t γ_r γ_m γ_mt γ_msy r -∗
+    thread_start Σ Hg1 Hg2 Hg3 γ_t γ_mt tid t0 -∗
+    □ update_helping_protocol Σ Hg1 Hg2 Hg3 N γ_t γ_r γ_mt γ_msy -∗ 
+    ⌜1 < L ∧ 0 < k < W⌝ -∗
+    ⌜i < L - 1⌝ -∗
+      {{{ traversal_inv Σ Hg1 Hg2 Hg3 γ_m t0 i k p pn
+          ∗ (∃ s, past_state Σ Hg1 Hg2 Hg3 γ_m t0 s ∗ ⌜c ∈ FP s ∧ i < Height s c⌝)
+          ∗ (⌜pn ≠ c⌝ -∗ past_marked_segment Σ Hg1 Hg2 Hg3 γ_m t0 i pn ls c) }}}
+        traverse_i #i #p #pn #c #k @ ⊤
+      {{{ (ores: option (Node * Node * bool)), 
+            RET (match ores with
+                  None => NONEV
+                | Some res =>SOMEV (#res.1.1,#res.1.2,#res.2) end);
+            match ores with 
+              None => True
+            | Some res =>
+              let p' := res.1.1 in let c' := res.1.2 in let b := res.2 in
+              traversal_inv Σ Hg1 Hg2 Hg3 γ_m t0 i k p' c'
+              ∗ (⌜i = 0⌝ → (∃ s, past_state Σ Hg1 Hg2 Hg3 γ_m t0 s ∗ 
+                              ⌜if b then 
+                                  k ∈ abs s ∧ k = Key s c' 
+                                  ∧ c' ∈ FP s ∧ Marki s c' 0 = false
+                                else 
+                                  k ∉ abs s ∧ k < Key s c' 
+                                  ∧ c' ∈ FP s⌝)) end }}}.
+  Proof.
+    iIntros "#HInv #Thd_st #Upd [%HL %Range_k] %HiL". 
+    iLöb as "IH" forall (p pn c ls). iIntros (Φ) "!# (#Htr & #FP_c & Hls) Hpost". 
+    wp_lam. wp_pure credit: "Hc". wp_pures. 
+    awp_apply findNext_spec.
+    iInv "HInv" as (M0 T0 s0) "(>Ds & >%Habs0 & >Hist & Help & >Templ)".
+    iDestruct "Templ" as (hd tl)"(HR & SShot0 & Res & %PT0 & %Trans_M0)".
+    iDestruct "Res" as "(GKS & Nodes & Nodes_KS)".
+    iAssert (⌜c ∈ FP s0⌝)%I as %FP_c0.
+    { apply leibniz_equiv in Habs0. rewrite -Habs0.
+      iDestruct "FP_c" as (s)"(Past_s & %FP_c & %Ht_c)".
+      iApply (in_FP_2 with "[%] [$Hist] [$Past_s] [%]"); try done. }
+    rewrite (big_sepS_delete _ (FP s0) c); last by eauto.
+    iDestruct "Nodes" as "(Node_c & Nodes_rest)".
+    iAssert (⌜i < Height s0 c⌝)%I as %Height_c0.
+    { apply leibniz_equiv in Habs0. rewrite -Habs0.
+      iDestruct "FP_c" as (s)"(Past_s & %FP_c & %Ht_c)".
+      iPoseProof (height_eq_2 Σ Hg1 Hg2 Hg3 c with "[%] [$] [$Past_s] [%]") as "->"; 
+        try done. }
+    iAssert ((node Σ c (Height s0 c) (Mark s0 c) (Next s0 c) (Key s0 c)) 
+      ∗ ⌜i < Height s0 c⌝)%I with "[Node_c]" as "Hpre".
+    { iFrame "Node_c %". }
+    iAaccIntro with "Hpre".
+    { iIntros "(Node_c & _)". iModIntro. iFrame "Hpost Hc Hls".
+      iNext; iExists M0, T0, s0. iFrame "∗%#". iExists hd, tl. iFrame "∗%#". 
+      rewrite (big_sepS_delete _ (FP s0) c); last by eauto. 
+      iFrame "Nodes_rest". iFrame. }
+    iIntros (m cn) "(Node_c & %Mark_c0 & %Next_c0)".
+    iAssert (⌜per_tick_inv hd tl s0⌝)%I as %PT_s0.
+    { iApply (per_tick_current with "[%] [%] [$Hist]"); try done. }
+    iPoseProof (snapshot_current with "[%] [#] [$]") 
+      as ">(#Past_s0&Hist)"; try done.
+    assert (c ≠ tl → Next s0 c !! i = Some cn) as Next_c0'. 
+    { intros Hctl. rewrite lookup_lookup_total. by rewrite Next_c0. 
+      rewrite -elem_of_dom. apply PT_s0 in FP_c0. destruct FP_c0 as (_&H'&H''). 
+      rewrite H'; try done. rewrite elem_of_gset_seq. lia. }
+    iAssert (⌜Mark s0 c !!! i = false⌝ → ⌜Key s0 c < k⌝ → 
+      traversal_inv Σ Hg1 Hg2 Hg3 γ_m t0 i k c cn)%I as "#Hcase".
+    { iIntros "%Hm %Hk". assert (Next s0 c !! i = Some cn) as H'. apply Next_c0'.
+      intros ->. destruct PT_s0 as ((_&_&H'&_)&_). clear -H' Hk Range_k. lia.
+      iSplitL; iExists s0; iFrame "Past_s0"; iPureIntro.
+      repeat split; try done. apply PT_s0 in FP_c0. destruct FP_c0 as (H''&_).
+      apply H''. by exists i. destruct PT_s0 as (_&_&_&_&_&PT&PT').
+      repeat split; try done. by apply (PT c _ i). by apply (PT' c _ i). }
+    
+    iAssert (⌜pn = c⌝ -∗ 
+              ∃ s, past_state Σ Hg1 Hg2 Hg3 γ_m t0 s
+            ∗ ⌜p ∈ FP s⌝
+            ∗ ⌜Key s p < k⌝
+            ∗ ⌜Marki s p 0 = false⌝
+            ∗ ⌜i < Height s p⌝
+            ∗ ⌜i = 0 → Nexti s p i = Some c⌝
+            ∗ ⌜per_tick_inv hd tl s⌝
+            ∗ ⌜c ∈ FP s → Mark s0 c !!! i = false → Mark s c !!! i = false⌝
+            ∗ ⌜c ∈ FP s → Key s c = Key s0 c⌝
+            ∗ ⌜∀ k, c ∈ FP s → k ∈ keyset (FI s c) → k ∈ abs s ↔ k ∈ Content s c⌝)%I
+      with "[Hist]" as "#Htr'".
+    { iIntros "%". subst pn. iDestruct "Htr" as "(Htrp & Htrc)".
+      iDestruct "Htrp" as (s)"(Past_s & %FP_ps & %Key_ps & %Marki_ps & 
+        %Height_ps & %Nexti_ps)".
+      iAssert (⌜per_tick_inv hd tl s⌝)%I as %PT_s.
+      { iPoseProof (per_tick_past with "[%] Hist Past_s") as "%"; try done. }
+      iAssert (⌜c ∈ FP s⌝ → ⌜Mark s0 c !!! i = false⌝ 
+        → ⌜Mark s c !!! i = false⌝)%I as %HM.
+      { iIntros "%FP_cs %Hm". destruct (decide (Mark s c !!! i = false)); try done.
+        iExFalso. rewrite not_false_iff_true in n.
+        iAssert (⌜Marki s0 c i = Marki s c i⌝)%I as %H'.
+        { apply leibniz_equiv in Habs0. rewrite -Habs0.
+          iPoseProof (marking_mono_2 Σ Hg1 Hg2 Hg3 c with "[%] [$Hist] [$Past_s] [%]") as "->"; 
+            try done. }
+        rewrite /Marki Hm n in H'. done. } 
+      iAssert (⌜c ∈ FP s⌝ → ⌜Key s c = Key s0 c⌝)%I as %Key_eq. 
+      { iIntros "%FP_cs". 
+        apply leibniz_equiv in Habs0. rewrite -Habs0.
+        iPoseProof (key_eq_2 Σ Hg1 Hg2 Hg3 c with "[%] [$Hist] [$Past_s] [%]") as "->"; 
+          try done. }
+      assert (∀ k, c ∈ FP s →  k ∈ keyset (FI s c) → 
+        (k ∈ abs s ↔ k ∈ Content s c)) as Hks.
+      { destruct PT_s as (_&_&H'&_). intros k'; apply H'. }
+      iExists s. iFrame "#%". }
+    iAssert (⌜pn = c⌝ -∗ ⌜i = 0⌝ → ⌜Mark s0 c !!! i = false⌝ → ⌜k < Key s0 c⌝ → 
+      ∃ s, past_state Σ Hg1 Hg2 Hg3 γ_m t0 s 
+          ∗ ⌜k ∉ abs s ∧ k < Key s c ∧ c ∈ FP s⌝)%I as "Hcase1".
+    { iIntros "%Hpnc %Hi %Mark_c0' %Key_c0".
+      iDestruct ("Htr'" with "[%]") as (s)"(#Past_s & %FP_ps & %Key_ps & %Marki_ps 
+        & %Height_ps & %Nexti_ps & %PT_s & %HM & %Key_eq & %Hks)"; try done.  
+      pose proof Nexti_ps Hi as Nexti_ps'.
+      subst i. iExists s. iFrame "Past_s". clear Nexti_ps.
+      assert (c ∈ FP s) as FP_cs. 
+      { destruct PT_s as (_&_&_&_&_&H'&_). apply (H' p c 0); try done. }
+      apply HM in Mark_c0'; try done. rename Mark_c0' into Mark_cs. 
+      rewrite -Key_eq in Key_c0; try done.
+      assert (k ∈ keyset (FI s c)) as k_in_ksc.
+      { apply (in_keyset hd tl s p c k); try done. lia. }
+      assert (k ∉ Content s c) as k_notin_cntc.
+      { rewrite /Content /Marki Mark_cs elem_of_singleton. lia. }
+      apply Hks in k_in_ksc; try done. iPureIntro. repeat split; try done.
+      intros H'%k_in_ksc. by apply k_notin_cntc. }
+    iAssert (⌜pn = c⌝ -∗ ⌜i = 0⌝ → ⌜Mark s0 c !!! i = false⌝ → ⌜k = Key s0 c⌝ → 
+      ∃ s, past_state Σ Hg1 Hg2 Hg3 γ_m t0 s 
+          ∗ ⌜k ∈ abs s ∧ k = Key s c ∧ c ∈ FP s ∧ Marki s c 0 = false⌝)%I as "Hcase2".
+    { iIntros "%Hpnc %Hi %Mark_c0' %Key_c0".
+      iDestruct ("Htr'" with "[%]") as (s)"(#Past_s & %FP_ps & %Key_ps & %Marki_ps 
+        & %Height_ps & %Nexti_ps & %PT_s & %HM & %Key_eq & %Hks)"; try done.
+      pose proof Nexti_ps Hi as Nexti_ps'.
+      subst i. iExists s. iFrame "Past_s". clear Nexti_ps. 
+      assert (c ∈ FP s) as FP_cs. 
+      { destruct PT_s as (_&_&_&_&_&H'&_). apply (H' p c 0); try done. }
+      apply HM in Mark_c0'; try done. rename Mark_c0' into Mark_cs. 
+      rewrite -Key_eq in Key_c0; try done.
+      assert (k ∈ keyset (FI s c)) as k_in_ksc.
+      { apply (in_keyset hd tl s p c k); try done. lia. }
+      assert (k ∈ Content s c) as k_in_cntc.
+      { rewrite /Content /Marki Mark_cs elem_of_singleton. lia. }
+      apply Hks in k_in_ksc; try done. iPureIntro. repeat split; try done.
+      by apply k_in_ksc. }
+    assert (m = true → c ≠ tl) as H1'.
+    { intros ->. destruct PT_s0 as ((_&_&_&_&H'&_)&_).
+      assert (i < L) as H'' by lia. pose proof H' i H'' as H1'.
+      intros ->. rewrite H1' in Mark_c0; try done. }
+    iAssert (⌜m = true⌝ → ∃ s, past_state Σ Hg1 Hg2 Hg3 γ_m t0 s 
+      ∗ ⌜cn ∈ FP s ∧ i < Height s cn⌝)%I as "#FP_cn'".
+    { iIntros "%". subst m. iExists s0. iFrame "Past_s0". iPureIntro. 
+      destruct PT_s0 as (_&_&_&_&_&H'&H''). split.
+      apply (H' c cn i). apply Next_c0'. by apply H1'. 
+      apply (H'' c cn i). apply Next_c0'. by apply H1'. }
+    iAssert (⌜m = true⌝ -∗ ∃ s : snapshot, past_state Σ Hg1 Hg2 Hg3 γ_m t0 s ∗
+      ⌜c ∈ FP s ∧ Marki s c i = true ∧ Nexti s c i = Some cn⌝)%I as "Hcase3'".
+    { iIntros "%". subst m. iExists s0. iFrame "Past_s0". iPureIntro.
+      repeat split; try done. apply Next_c0'. by apply H1'. }
+
+    iModIntro. iSplitR "Hpost Hc Hls".
+    { iNext. iExists M0, T0, s0. iFrame "∗%". iExists hd, tl. iFrame "∗%".
+      rewrite (big_sepS_delete _ (FP s0) c); last by eauto.
+      iFrame "Nodes_rest". iFrame. }
+    clear Habs0 PT0 Trans_M0 PT_s0 Next_c0' H1'.
+
+    destruct m; wp_pures.
+    { iDestruct ("FP_cn'" with "[%]") as "FP_cn"; try done.
+      iDestruct ("Hcase3'" with "[%]") as "Hcase3"; try done.
+      destruct (decide (pn = c)) as [-> | Hpnc].
+      iApply ("IH" $! p c cn []); try done. iFrame "Htr FP_cn".
+      iIntros "%". rewrite /past_marked_segment. iApply "Hcase3"; try done.
+      iDestruct ("Hls" with "[%]") as "Hls"; try done.
+      iAssert (past_marked_segment Σ Hg1 Hg2 Hg3 γ_m t0 i pn (ls ++ [c]) cn)
+        with "[Hls]" as "Hls".
+      { rewrite /past_marked_segment. 
+        destruct ls as [| n lss] eqn: Def_ls. 
+        - iSimpl. iFrame "Hls". iSplit. iIntros (j)"%H'". exfalso. clear -H'; lia.
+          iApply "Hcase3"; try done.
+        - iSimpl. iDestruct "Hls" as "(Hls1 & Hls2 & Hls3)".
+          iFrame "Hls1". iSplit.
+          + iIntros (j)"%Hj". rewrite app_length /= in Hj. 
+            destruct (decide (j = length lss)) as [-> | Hj'].
+            assert ((n :: lss ++ [c]) !!! length lss = 
+              (n :: lss) !!! (length (n :: lss) - 1)) as ->.
+            { rewrite /=. rewrite (lookup_total_app_l (n :: lss) [c]). 
+              rewrite Nat.sub_0_r. done. rewrite /=. lia. }
+            assert ((n :: lss ++ [c]) !!! (length lss + 1)%nat = c) as ->.
+            { assert (length lss + 1 = length (n :: lss)) as ->.
+              { rewrite /=. lia. } 
+              rewrite (list_lookup_total_middle (n :: lss)); try done. }
+            iFrame "Hls3".
+            assert ((n :: lss ++ [c]) !!! j = (n :: lss) !!! j) as ->.
+            { rewrite (lookup_total_app_l (n :: lss) [c]). done.
+              rewrite /=; lia. }
+            assert ((n :: lss ++ [c]) !!! (j + 1)%nat = 
+              (n :: lss) !!! (j + 1)%nat) as ->.
+            { rewrite (lookup_total_app_l (n :: lss) [c]). done.
+              rewrite /=; lia. }
+            iApply "Hls2". iPureIntro. 
+            assert (length (lss ++ [c]) = length lss + 1) as H'.
+            { by rewrite app_length /=. }
+            rewrite /=. lia.
+          + assert ((n :: lss ++ [c]) !!! (length (lss ++ [c]) - 0) = c) as ->.
+            { rewrite app_length /=. 
+            rewrite (list_lookup_total_middle (n :: lss)); try done.
+            rewrite /=; lia. }
+            iApply "Hcase3"; try done. }
+      iSpecialize ("IH" $! p pn cn (ls ++ [c])).
+      iApply ("IH" with "[Hls]"); try done. iFrame "Htr FP_cn".
+      iIntros "%". done. }
+    awp_apply compareKey_spec. 
+    iInv "HInv" as (M1 T1 s1) "(>Ds & >%Habs1 & >Hist & Help & >Templ)".
+    iDestruct "Templ" as (hd' tl')"(HR & SShot1 & Res & %PT1 & %Trans_M1)".
+    iAssert (⌜hd' = hd ∧ tl' = tl⌝)%I as %[-> ->]. admit.
+    iDestruct "Res" as "(GKS & Nodes & Nodes_KS)".
+    iAssert (⌜c ∈ FP s1⌝)%I as %FP_c1.
+    { apply leibniz_equiv in Habs1. rewrite -Habs1.
+      iApply (in_FP_2 with "[%] [$Hist] [$Past_s0] [%]"); try done. }
+    rewrite (big_sepS_delete _ (FP s1) c); last by eauto.
+    iDestruct "Nodes" as "(Node_c & Nodes_rest)".
+    iAaccIntro with "Node_c".
+    { iIntros "Node_c". iModIntro. iFrame "Hpost Hc Hls".
+      iNext; iExists M1, T1, s1. iFrame "∗%#". iExists hd, tl. iFrame "∗%#".
+      rewrite (big_sepS_delete _ (FP s1) c); last by eauto. iFrame. }
+    iIntros (res)"(Node_c & %Hif)".
+    iPoseProof (snapshot_current with "[%] [#] [$Hist]") 
+          as ">(#Past_s1&Hist)"; try done.
+    iAssert (⌜Key s1 c = Key s0 c⌝)%I as %Key_c10.
+    { apply leibniz_equiv in Habs1. rewrite -Habs1.
+      iPoseProof (key_eq_2 with "[%] [$Hist] [$Past_s0] [%]") as "->"; try done. }
+    iModIntro. iSplitR "Hpost Hls".
+    { iNext. iExists M1, T1, s1. iFrame "∗%". iExists hd, tl. iFrame "∗%".
+      rewrite (big_sepS_delete _ (FP s1) c); last by eauto.
+      iFrame "Nodes_rest". iFrame. }
+    clear Habs1 PT1 Trans_M1.
+    wp_pures.
+    destruct (bool_decide (#res = #0)) eqn: Hbool.
+    { wp_pures. iApply ("IH" $! c cn cn []); try done.
+      assert (Key s0 c < k) as H'.
+      { rewrite -Key_c10. rewrite bool_decide_eq_true in Hbool.
+        inversion Hbool. rewrite decide_True in Hif; last first.
+        clear -H0; lia. done. }
+      iDestruct ("Hcase" with "[%] [%]") as "H'"; try done.
+      iFrame "H'". iDestruct "H'" as "(_&H')". iFrame "H'".
+      iIntros "%"; try done. }
+    rewrite bool_decide_eq_false in Hbool.
+    assert (res ≠ 0) as res_neq_0. 
+    { intros ->. apply Hbool. apply f_equal. apply f_equal. lia. }
+    wp_pures. destruct (bool_decide (#pn = #c)) eqn: Hpnc.
+    - rewrite bool_decide_eq_true in Hpnc. inversion Hpnc. subst pn.
+      wp_pures. destruct (bool_decide (#res = #1)) eqn:Hbool1.
+      + wp_pures. iApply ("Hpost" $! (Some (p, c, true))). iSimpl.
+        iModIntro. iFrame "Htr". iIntros "%Hi0". iApply "Hcase2"; try done.
+        iPureIntro. rewrite bool_decide_eq_true in Hbool1.
+        inversion Hbool1. rewrite decide_False in Hif; try done.
+        rewrite decide_True in Hif; try lia.
+      + wp_pures. iApply ("Hpost" $! (Some (p, c, false))). iSimpl.
+        iModIntro. iFrame "Htr". iIntros "%Hi0". iApply "Hcase1"; try done.
+        iPureIntro. rewrite bool_decide_eq_false in Hbool1.
+        rewrite decide_False in Hif; try done.
+        rewrite decide_False in Hif; try lia. intros ->. apply Hbool1. 
+        apply f_equal. apply f_equal. lia.
+    - iClear "Hcase Htr' Hcase1 Hcase2 FP_cn' Hcase3' Past_s0".
+      wp_pure credit: "Hc". wp_pures. awp_apply changeNext_spec; try done.
+      iInv "HInv" as (M2 T2 s2) "(>Ds & >%Habs2 & >Hist & Help & >Templ)".
+      iDestruct "Templ" as (hd' tl')"(HR & SShot2 & Res & %PT2 & %Trans_M2)".
+      iAssert (⌜hd' = hd ∧ tl' = tl⌝)%I as %[-> ->]. admit.
+      iDestruct "Res" as "(GKS & Nodes & Nodes_KS)".
+      iPoseProof (snapshot_current with "[%] [#] [$]") 
+        as ">(#Past_s2&Hist)"; try done.
+      iAssert (⌜p ∈ FP s2⌝)%I as %FP_p2.
+      { apply leibniz_equiv in Habs2. rewrite -Habs2.
+        iDestruct "Htr" as "(H'&_)". iDestruct "H'" as (s)"(Past_s & %Htr_sp)".
+        destruct Htr_sp as (H'&_). 
+        iApply (in_FP_2 with "[%] [$Hist] [$Past_s] [%]"); try done. }
+      rewrite (big_sepS_delete _ (FP s2) p); last by eauto.
+      iDestruct "Nodes" as "(Node_p & Nodes_rest)".
+      iAssert (⌜i < Height s2 p⌝)%I as %Height_p2.
+      { apply leibniz_equiv in Habs2. rewrite -Habs2.
+        iDestruct "Htr" as "(H'&_)". iDestruct "H'" as (s)"(Past_s & %Htr_sp)".
+        destruct Htr_sp as (H'&_&_&H''&_). 
+        iPoseProof (height_eq_2 _ _ _ _ p with "[%] [$Hist] [$Past_s] [%]") as "->"; 
+          try done. }
+      iAssert ((node _ p (Height s2 p) (Mark s2 p) (Next s2 p) (Key s2 p)) 
+        ∗ ⌜i < Height s2 p⌝)%I with "[Node_p]" as "Hpre".
+      { iFrame "Node_p %". }
+      iAaccIntro with "Hpre".
+      { iIntros "(Node_p&_)". iModIntro. iFrame "Hpost Hc Hls".
+        iNext; iExists M2, T2, s2. iFrame "∗%#". iExists hd, tl. iFrame "∗%#". 
+        rewrite (big_sepS_delete _ (FP s2) p); last by eauto. iFrame. }
+      iIntros (success next') "(Node_p & Hsuccess)".
+      iApply (lc_fupd_add_later with "Hc"). iNext. 
+      destruct success; last first.
+      { iDestruct "Hsuccess" as %(_&->).
+        iModIntro. iSplitR "Hpost Hls".
+        { iNext. iExists M2, T2, s2. iFrame "∗%". iExists hd, tl. iFrame "∗%".
+          rewrite (big_sepS_delete _ (FP s2) p); last by eauto.
+          iFrame "Nodes_rest". iFrame. }
+        wp_pures. iApply ("Hpost" $! None). done. }
+      
+      iDestruct "Hsuccess" as %[Next_p2' [Mark_p2 Def_next']].
+      assert (pn ≠ c) as pn_neq_c.
+      { intros <-. rewrite bool_decide_eq_false in Hpnc. by apply Hpnc. }
+      iDestruct ("Hls" with "[%]") as "Hls"; try done.
+      (*
+      destruct ls as [| pnn lss] eqn: Def_ls. 
+      { iDestruct "Hls" as %H'. clear -H' pn_neq_c; done. }
+      rewrite <-Def_ls. iDestruct "Hls" as "#Hls". 
+      *)
+      iAssert (⌜per_tick_inv hd tl s2⌝)%I as %PT_s2.
+      { iApply (per_tick_current with "[%] [%] [$Hist]"); try done. }
+
+      iAssert (⌜Key s2 p < k⌝)%I as %Key_pk. 
+      { apply leibniz_equiv in Habs2. rewrite -Habs2.
+        iDestruct "Htr" as "(H'&_)". iDestruct "H'" as (s)"(Past_s & %Htr_sp)".
+        destruct Htr_sp as (H'&H''&_).
+        iPoseProof (key_eq_2 _ _ _ _ p with "[%] [$Hist] [$Past_s] [%]") as "->"; 
+          try done. }
+      assert (Key s2 p < W) as Key_pW. { clear -Key_pk Range_k; lia. }
+      assert (p ≠ tl) as p_neq_tl.
+      { intros ->. destruct PT_s2 as ((_&_&H'&_)&_). clear -H' Key_pk Range_k; lia. }
+      iAssert (⌜Key s2 c = Key s1 c⌝)%I as %Key_c21.
+      { apply leibniz_equiv in Habs2. rewrite -Habs2.
+        iPoseProof (key_eq_2 _ _ _ _ c with "[%] [$Hist] [$Past_s1] [%]") as "->"; 
+          try done. }
+
+      assert (Next s2 p !! i = Some pn) as Next_p2.
+      { rewrite lookup_lookup_total. by rewrite Next_p2'. rewrite -elem_of_dom.
+        apply PT_s2 in FP_p2. destruct FP_p2 as (_&H'&_). rewrite H'.
+        rewrite elem_of_gset_seq. lia. done. }
+      
+      iAssert (⌜Marki s2 pn i = true⌝)%I as %Marki_pn2.
+      { rewrite /past_marked_segment. destruct ls as [ | n lss] eqn: Def_ls. 
+        iDestruct "Hls" as (s)"(Past_s & %FP_pn & %Mark_pn & _)".
+        apply leibniz_equiv in Habs2. rewrite -Habs2.
+        iPoseProof (marking_mono_2 _ _ _ _ pn with "[%] [$Hist] [$Past_s] [%]") 
+          as "->"; try done.
+        rewrite <-Def_ls.
+        iDestruct "Hls" as "(H'&_)". 
+        iDestruct "H'" as (s)"(Past_s & %FP_pn & %Mark_pn & _)".
+        apply leibniz_equiv in Habs2. rewrite -Habs2.
+        iPoseProof (marking_mono_2 _ _ _ _ pn with "[%] [$Hist] [$Past_s] [%]") 
+          as "->"; try done. }
+      iAssert (∀ n, ⌜n ∈ ls⌝ → ⌜Marki s2 n i = true⌝)%I as %Marki_ls.
+      { rewrite /past_marked_segment. destruct ls as [ | n0 lss] eqn: Def_ls.
+        iIntros (n)"%H'"; clear -H'; set_solver.
+        rewrite <-Def_ls.
+        iIntros (n)"%Hn". assert (Hn' := Hn). 
+        apply elem_of_list_lookup_total in Hn'. destruct Hn' as [j [Hj Def_j]].
+        destruct (decide (j = length ls - 1)) as [-> | Hlj].
+        - iDestruct "Hls" as "(_&_&H')". 
+          iDestruct "H'" as (s)"(Past_s & %FP_n & %Mark_n & _)".
+          apply leibniz_equiv in Habs2. rewrite -Habs2.
+          iPoseProof (marking_mono_2 _ _ _ _ n with "[%] [$Hist] [$Past_s] [%]") 
+            as "->"; try done. all: by rewrite -Def_j.
+        - assert (j < length ls - 1) as Hj'. { clear - Hlj Hj. lia. }
+          iDestruct "Hls" as "(_&H'&_)".
+          iDestruct ("H'" with "[%]") as "H''". apply Hj'.
+        iDestruct "H''" as (s)"(Past_s & %FP_n & %Mark_n & _)".
+        apply leibniz_equiv in Habs2. rewrite -Habs2.
+        iPoseProof (marking_mono_2 _ _ _ _ n with "[%] [$Hist] [$Past_s] [%]") as "->"; 
+          try done. all: by rewrite -Def_j. }
+      iAssert (⌜ls = []⌝ -∗ ⌜Nexti s2 pn i = Some c⌝)%I as %Nexti_pn2.
+      { iIntros "%". subst ls.
+        iDestruct "Hls" as (s)"(Past_s & %FP_pn & %Mark_pn & %Next_pn)".
+        apply leibniz_equiv in Habs2. rewrite -Habs2.
+        iPoseProof (next_unchanged _ _ _ _ pn with "[%] [$Hist] [$Past_s] [%]") 
+          as "->"; try done. }
+      iAssert (∀ pnn lss, ⌜ls = pnn :: lss⌝ -∗ 
+        ⌜Nexti s2 pn i = Some pnn⌝)%I as %Nexti_pn2'.
+      { iIntros (pnn lss)"%". subst ls.
+        iDestruct "Hls" as "(Hls&_)". 
+        iDestruct "Hls" as (s)"(Past_s & %FP_pn & %Mark_pn & %Next_pn)".
+        apply leibniz_equiv in Habs2. rewrite -Habs2.
+        iPoseProof (next_unchanged _ _ _ _ pn with "[%] [$Hist] [$Past_s] [%]") 
+          as "->"; try done. }
+      iAssert (∀ j, ⌜j < length ls - 1⌝ → 
+        ⌜Nexti s2 (ls !!! j) i = Some (ls !!! (j+1)%nat)⌝)%I as %Nexti_ls.
+      { rewrite /past_marked_segment. destruct ls as [ | n0 lss] eqn: Def_ls.
+        iIntros (j)"%H'"; clear -H'. exfalso. rewrite /= in H'. lia.
+        rewrite <-Def_ls.
+        iIntros (j)"%Hj". iDestruct "Hls" as "(_&H'&_)". 
+        iDestruct ("H'" with "[%]") as "H''". apply Hj.
+        iDestruct "H''" as (s)"(Past_s & %FP_n & %Mark_n & %Next_n)".
+        apply leibniz_equiv in Habs2. rewrite -Habs2.
+        iPoseProof (next_unchanged _ _ _ _ (ls !!! j) with "[%] [$Hist] [$Past_s] [%]") 
+          as "->"; try done. }
+      iAssert (∀ pnn lss, ⌜ls = pnn :: lss⌝ -∗
+        ⌜Nexti s2 (ls !!! (length ls - 1)) i = Some c⌝)%I as %Nexti_lsc.
+      { iIntros (pnn lss)"%". subst ls. iDestruct "Hls" as "(_&_&H')". 
+        iDestruct "H'" as (s)"(Past_s & %FP_n & %Mark_n & %Next_n)".
+        apply leibniz_equiv in Habs2. rewrite -Habs2.
+        iPoseProof (next_unchanged _ _ _ _ _ with "[%] [$Hist] [$Past_s] [%]") 
+          as "->"; try done. }
+      iAssert (⌜c ∈ FP s2⌝)%I as %FP_c2. 
+      { apply leibniz_equiv in Habs2. rewrite -Habs2.
+        iDestruct "FP_c" as (s)"(Past_s & %FP_c & %Ht_c)".
+        iApply (in_FP_2 with "[%] [$Hist] [$Past_s] [%]"); try done. }
+      iAssert (⌜i < Height s2 c⌝)%I as %Ht_c2. 
+      { apply leibniz_equiv in Habs2. rewrite -Habs2.
+        iDestruct "FP_c" as (s)"(Past_s & %FP_c & %Ht_c)".
+        iPoseProof (height_eq_2 Σ Hg1 Hg2 Hg3 c with "[%] [$] [$Past_s] [%]") as "->"; 
+          try done. }
+
+      destruct (decide (i = 0)) as [-> | Hi0].
+      + iDestruct "SShot2" as %[FP2 [C2 [Ht2 [Mk2 [Nx2 [Ky2 [I2 
+          [Hs2 [Dom_Ht2 [Dom_Mk2 [Dom_Nx2 [Dom_Ky2 Dom_I2]]]]]]]]]]]].
+        assert (∀ x, x ∈ FP s2 → flow_constraints_I x (FI s2 x) 
+              (Mark s2 x !!! 0) (Next s2 x !! 0) (Key s2 x)) as Hflow.
+        { destruct PT_s2 as (_&_&_&H'&_).
+          intros x Hx. apply H' in Hx. by destruct Hx as (_&_&_&_&_&?). }
+        assert (∀ x, I2 !!! x = FI s2 x) as I2_eq_s2.
+        { intros x. rewrite Hs2; unfold FI. try done. }
+        assert (p ∈ dom I2) as p_in_I2. { by rewrite Hs2 /= -Dom_I2 in FP_p2. }
+        
+
+        iAssert (⌜∃ (I: gmap Node (multiset_flowint_ur nat)),
+                    dom I = {[p; pn]} ∪ list_to_set ls
+                  ∧ dom I ⊆ dom I2
+                  ∧ Key s2 p < Key s2 c
+                  ∧ ([^op set] x ∈ dom I, FI s2 x) = ([^op set] x ∈ dom I, I !!! x)
+                  ∧ (I !!! p = int {| infR := inf_map (FI s2 p); 
+                                  outR := <<[ c := out (FI s2 p) pn ]>> ∅ |})
+                  ∧ (∀ x, x ∈ dom I → x ≠ p → 
+                      I !!! x = int {| infR := {[x := ∅]}; outR := ∅ |})
+                  ∧ (flow_constraints_I p (I !!! p) (Mark s2 p !!! 0)
+                      (Some c) (Key s2 p))
+                  ∧ (∀ x, x ∈ dom I → x ≠ p → flow_constraints_I x (I !!! x) 
+                      (Mark s2 x !!! 0) (Next s2 x !! 0) (Key s2 x))
+                  ∧ (∀ x, x ∈ dom I → keyset (I !!! x) = keyset (I2 !!! x))⌝)%I 
+          as %[I Hflupd].
+        { assert (∃ (Nx: gmap Node Node), ∀ x, Nx !! x = Next s2 x !! 0)
+            as [Nx Def_Nx].
+          { admit. }
+          assert (∃ (Mk: gmap Node bool), ∀ (x: Node), Mk !! x = Mark s2 x !! 0)
+            as [Mk Def_Mk'].
+          { admit. }
+          assert (∀ x, Mk !!! x = Mark s2 x !!! 0) as Def_Mk.
+          { intros n. rewrite lookup_total_alt. by rewrite Def_Mk'. }
+          assert (dom Nx ⊆ dom Nx2) as Dom_Nx.
+          { intros n. rewrite !elem_of_dom. rewrite Def_Nx.
+            rewrite Hs2. unfold Nexti, Next.
+            destruct (Nx2 !! n) eqn: H'; try done.
+            rewrite H'. rewrite lookup_empty. 
+            intros [? H'']; try done. }
+          assert (dom Mk = dom Mk2) as Dom_Mk.
+          { apply set_eq_subseteq; split.
+            - intros n. rewrite !elem_of_dom. rewrite Def_Mk'.
+              rewrite Hs2. unfold Mark.
+              destruct (Mk2 !! n) eqn: H'; try done.
+              rewrite H'. rewrite lookup_empty. 
+              intros [? H'']; try done.
+            - intros n. rewrite !elem_of_dom. rewrite Def_Mk'.
+              rewrite Hs2. unfold Mark.
+              destruct (Mk2 !! n) eqn: H'; try done.
+              rewrite H'. intros _.
+              assert (H1' := H'). 
+              apply elem_of_dom_2 in H'.
+              rewrite Dom_Mk2 in H'.
+              destruct PT_s2 as (_&_&_&PT&_).
+              rewrite {1}Hs2 in PT. unfold FP in PT.
+              apply PT in H'. destruct H' as (_&_&H'&_).
+              rewrite Hs2 /Mark H1' in H'.
+              rewrite -elem_of_dom H' elem_of_gset_seq. clear; lia.
+              intros [? H'']; try done. }
+          assert (∀ x, Ky2 !!! x = Key s2 x) as Def_Ky2.
+          { rewrite Hs2. unfold Key. try done. }
+
+          assert (nx_key_rel Nx Ky2) as Nx_key_rel.
+          { destruct PT_s2 as (_&_&_&_&H'&_). intros n1 n2.
+            rewrite !Def_Nx !Def_Ky2. apply H'. }
+          assert (nx_mk_closed Nx Mk (dom I2)) as Hcl.
+          { split; last split; last split. 
+            - rewrite Dom_I2 -Dom_Nx2. done.
+            - rewrite Dom_Mk. clear -Dom_Mk2 Dom_I2; set_solver.
+            - destruct PT_s2 as (_&_&_&_&_&H'&_). intros n1 n2.
+              rewrite {2}Hs2 in H'. unfold FP in H'.
+              rewrite !Def_Nx Dom_I2. apply H'.
+            - intros x Hmx Hnx.
+              assert (x ∈ FP s2) as H'. rewrite /FP Hs2 -Dom_Mk2.
+              apply elem_of_dom_2 in Hmx. by rewrite -Dom_Mk.
+              apply PT_s2 in H'. destruct H' as (_&H'&_).
+              destruct (decide (x = tl)) as [-> | Hxtl].
+              + destruct PT_s2 as ((_&_&_&_&H''&_)&_).
+                pose proof H'' 0 as H''. rewrite -Def_Mk in H''; try done.
+                apply lookup_total_correct in Hmx. rewrite Hmx in H''.
+                clear -H'' HL; try (done || lia).
+              + apply H' in Hxtl. 
+                rewrite Def_Nx in Hnx; try done. 
+                rewrite -not_elem_of_dom Hxtl in Hnx. apply Hnx.
+                rewrite elem_of_gset_seq. clear; lia. }
+          assert (marked_segment Nx Mk pn ls c) as Hms.
+          { rewrite /marked_segment. repeat split.
+            rewrite Def_Mk. by rewrite /Marki in Marki_pn2.
+            intros x. rewrite Def_Mk. rewrite /Marki in Marki_ls. apply Marki_ls.
+            destruct ls as [ | pnn lss] eqn: Def_ls. 
+            rewrite /= Def_Nx. by apply Nexti_pn2.
+            repeat split. rewrite Def_Nx. by apply (Nexti_pn2' pnn lss).  
+            intros x. rewrite Def_Nx. rewrite /Nexti in Nexti_ls. apply Nexti_ls.
+            rewrite Def_Nx. by apply (Nexti_lsc pnn lss). }
+          clear Nexti_lsc Nexti_ls Nexti_pn2 Nexti_pn2'.
+          assert (✓ ([^op set] x ∈ dom I2, (I2 !!! x: multiset_flowint_ur nat))) 
+            as VI.
+          { destruct PT_s2 as (_&H'&_).
+            unfold GFI in H'. rewrite Dom_I2.
+            rewrite {2}Hs2 in H'. unfold FP in H'.
+            assert (([^op set] x ∈ FP2, I2 !!! x) = 
+              ([^op set] x ∈ FP2, FI s2 x)) as H1'.
+            { by apply big_opS_ext. }
+            by rewrite H1'. }
+          assert (FP s2 = dom I2) as FP_s2_I2.
+          { by rewrite /FP Hs2 Dom_I2. }
+          rewrite FP_s2_I2 in Hflow.
+          assert (∀ x, x ∈ dom I2 → dom (I2 !!! x: multiset_flowint_ur nat) 
+            = {[x]}) as Domm_I2.
+          { intros x Hx%Hflow. destruct Hx as (Hx&_). by rewrite I2_eq_s2. }
+          assert (∀ x, x ∈ dom I2 → Mk !!! x = true → 
+            keyset (I2 !!! x) = ∅) as KS_mk.
+          { intros x Hx%Hflow. rewrite Def_Mk I2_eq_s2. 
+            rewrite /Marki; intros H'; rewrite H' in Hx. 
+            by destruct Hx as (_&_&_&Hx&_). }
+          assert (∀ n1 n2, insets (I2 !!! n1) ≠ ∅ → Nx !! n1 = Some n2 → 
+            dom (out_map (I2 !!! n1: multiset_flowint_ur nat)) = {[n2]}) 
+            as Nx_dom.
+          { intros n1 n2 Hin Nx_n1. assert (n1 ∈ dom I2) as H'.
+            { apply elem_of_dom_2 in Nx_n1. apply Dom_Nx in Nx_n1. 
+              by rewrite Dom_I2 -Dom_Nx2. }
+            apply Hflow in H'. destruct H' as (_&H'&_).
+            rewrite -Def_Nx Nx_n1 -I2_eq_s2 in H'. by apply H' in Hin. }
+          assert (∀ x k, x ∈ dom I2 → 
+            inf ((I2 !!! x):multiset_flowint_ur _) x !!! k ≤ 1) as Inf_x.
+          { intros x k' Hx%Hflow. destruct Hx as (_&_&_&_&_&H'&_).
+            rewrite I2_eq_s2. apply H'. }
+          assert (∀ x x' k, x ∈ dom I2 → 
+            out ((I2 !!! x):multiset_flowint_ur _) x' !!! k ≤ 1) as Out_x.
+          { intros x x' k' Hx%Hflow. destruct Hx as (_&_&_&_&_&_&H').
+            rewrite I2_eq_s2. apply H'. }
+          assert (∀ x, x ∈ dom I2 → outsets (I2 !!! x) ⊆ insets (I2 !!! x))
+            as Out_In.
+          { intros x Hx%Hflow. destruct Hx as (_&_&H'&_).
+            rewrite I2_eq_s2. apply H'. }
+          
+          
+          assert (insets (I2 !!! p) ≠ ∅) as Insets_p_ne.
+          { apply Hflow in p_in_I2. rewrite -I2_eq_s2 Mark_p2 in p_in_I2.
+            destruct p_in_I2 as (_&_&_&(H'&_)&_).
+            apply (non_empty_inhabited_L k). apply H'.
+            rewrite elem_of_gset_seq. clear -Range_k Key_pk; lia. }
+          assert (Nx !! p = Some pn) as Nx_p.
+          { by rewrite Def_Nx. }
+          set S : nzmap nat nat := out (I2 !!! p) pn.
+          assert (W ∈ outset _ (I2 !!! p) pn) as Outset_W.
+          { apply Hflow in p_in_I2. rewrite -I2_eq_s2 Mark_p2 in p_in_I2.
+            assert (W ∈ outsets (I2 !!! p)) as H'.
+            { destruct p_in_I2 as (_&_&_&(_&H')&_). rewrite -H' elem_of_gset_seq.
+              split; try done. clear -Key_pW; lia. }
+            rewrite /outsets in H'. destruct p_in_I2 as (_&H''&_).
+            apply H'' in Insets_p_ne. rewrite Next_p2 in Insets_p_ne.
+            by rewrite Insets_p_ne big_opS_singleton in H'. }
+          assert (dom S ≠ ∅) as Dom_S.
+          { rewrite /S. rewrite /outset in Outset_W. clear -Outset_W; set_solver. }
+          assert (∀ x y, Nx !! x = Some y → 
+            insets ((I2 !!! x: multiset_flowint_ur nat)) ≠ ∅ → 
+              inf ((I2 !!! y : multiset_flowint_ur nat)) y = 
+              out ((I2 !!! x: multiset_flowint_ur nat)) y) as Inf_eq_Out.
+          { intros x y Nx_x Insets_x. rewrite !I2_eq_s2.
+            assert (x ∈ dom I2) as x_in_I2.
+            { apply elem_of_dom_2 in Nx_x. apply Hcl in Nx_x. done. }
+            assert (y ∈ dom I2) as y_in_I2.
+            { destruct Hcl as (_&_&H'&_). apply (H' x). done. }
+            rewrite I2_eq_s2 in Insets_x.
+            apply (outflow_eq_inflow hd tl); try done.
+            all: try (by rewrite FP_s2_I2). rewrite Def_Nx in Nx_x. apply Nx_x. }
+          set I' := list_flow_upd_unlink p pn ls c S Nx Mk I2.
+          assert (list_flow_upd_unlink p pn ls c S Nx Mk I2 = I') as Def_I'.
+          { by rewrite /I'. }
+
+          pose proof unlink_flow_upd_summary Ky2 p pn ls c Nx Mk I2 I'
+            Nx_key_rel Hcl Hms Dom_S Nx_p VI Domm_I2 Nx_dom KS_mk Inf_eq_Out 
+            Out_In Inf_x Out_x Insets_p_ne Def_I' as Hflupd.
+          destruct Hflupd as (Dom_I'&Dom_I'_in_I2&Ky_pc&Heq&I'_p&I'_x).
+          iPureIntro. exists I'. 
+          
+          assert (insets (I' !!! p) = insets (I2 !!! p)) as Insets_p.
+          { rewrite I'_p. clear. 
+            rewrite /insets /dom /flowint_dom /inset /inf /=. done. }
+          assert (outsets (I' !!! p) = outsets (I2 !!! p)) as Outsets_p.
+          { apply Nx_dom in Nx_p; try done. rewrite /outsets Nx_p.
+            assert (dom (out_map (I' !!! p : multiset_flowint_ur _)) = {[c]}) as H'.
+            { rewrite I'_p. rewrite /= -leibniz_equiv_iff nzmap_dom_insert_nonzero.
+              rewrite /dom; clear; set_solver. rewrite -/S. intros ->.
+              clear -Dom_S. rewrite /ccmunit /= in Dom_S. set_solver. }
+            rewrite H' -leibniz_equiv_iff !big_opS_singleton.
+            by rewrite /outset I'_p /out /= nzmap_lookup_total_insert. }
+          assert (∀ x, x ∈ dom I' → x ≠ p → insets (I' !!! x) = ∅) as Insets_x.
+          { intros x Hx Hxp. rewrite I'_x; try done. clear.
+            rewrite /insets /dom /flowint_dom /= dom_singleton_L.
+            rewrite -leibniz_equiv_iff big_opS_singleton.
+            rewrite /inset /inf /= lookup_insert /=. set_solver. }
+          assert (∀ x, x ∈ dom I' → x ≠ p → outsets (I' !!! x) = ∅) as Outsets_x.
+          { intros x Hx Hxp. rewrite I'_x; try done. clear. rewrite /outsets /=.
+            assert (dom ∅ = (∅: gset Node)) as ->. set_solver. 
+            rewrite big_opS_empty. set_solver. }
+          split; last split; last split; last split; last split; 
+            last split; last split; last split; try done.
+          - by rewrite !Def_Ky2 in Ky_pc.
+          - by rewrite Hs2 Heq. 
+          - by rewrite I'_p I2_eq_s2.
+          - assert (flow_constraints_I p (I2 !!! p) (false) (Some pn) (Key s2 p))
+              as Hp. 
+            { apply Hflow in p_in_I2. 
+              by rewrite -I2_eq_s2 Mark_p2 Next_p2 in p_in_I2. }
+            rewrite Mark_p2 I'_p. repeat split.
+            + rewrite /= /flowint_dom /=. by apply Domm_I2.
+            + intros ?. rewrite /= -leibniz_equiv_iff nzmap_dom_insert_nonzero.
+              rewrite /dom; clear; set_solver. rewrite -/S. intros ->.
+              clear -Dom_S. rewrite /ccmunit /= in Dom_S. set_solver.
+            + rewrite -I'_p Insets_p Outsets_p. apply Hp.
+            + rewrite -I'_p Insets_p. apply Hp. 
+            + rewrite -I'_p Outsets_p. apply Hp.
+            + rewrite -I'_p Insets_p. apply Hp.
+            + intros ?; rewrite /=; apply Hp.
+            + intros n k'; rewrite /out /=.
+              destruct (decide (n = c)) as [-> | Hnc].
+              rewrite nzmap_lookup_total_insert. apply Hp.
+              rewrite nzmap_lookup_total_insert_ne; try done. 
+              rewrite !nzmap_lookup_empty /ccmunit /= /nat_unit; clear; lia.
+          - intros x Hx Hxp. 
+            assert (Mark s2 x !!! 0 = true) as ->.
+            { rewrite Dom_I' !elem_of_union !elem_of_singleton in Hx. 
+              destruct Hx as [[-> | ->] | Hx]; try done. apply Marki_ls.
+              clear - Hx; set_solver. }
+            repeat split.
+            + rewrite I'_x; try done. 
+              rewrite /dom /flowint_dom /=. clear; set_solver.
+            + rewrite Insets_x; try done.
+            + rewrite Insets_x; try done. rewrite Outsets_x; try done.
+            + rewrite /keyset. rewrite Insets_x; try done. 
+              rewrite Outsets_x; try done.
+            + rewrite Insets_x; try done. 
+            + intros ?; rewrite I'_x; try done. rewrite /inf /= lookup_insert /=.
+              rewrite nzmap_lookup_empty /ccmunit /= /nat_unit. clear; lia.
+            + intros n k'; rewrite /out /out_map /=. rewrite I'_x /=; try done.
+              rewrite !nzmap_lookup_empty /ccmunit /= /nat_unit; clear; lia.
+          - intros x Hx. destruct (decide (x = p)) as [-> | Hxp].
+            + by rewrite /keyset Insets_p Outsets_p.
+            + assert (H' := Hx). rewrite Dom_I' in Hx.
+              assert (Mk !!! x = true) as Hmkx.
+              { clear -Hxp Hx Hms. destruct Hms as (Hm1&Hm2&_).
+                destruct (decide (x = pn)) as [-> | Hxpn]; try done.
+                apply Hm2. set_solver. }
+              apply KS_mk in Hmkx. rewrite Hmkx.
+              rewrite /keyset Insets_x; try done. rewrite Outsets_x; try done.
+              by apply Dom_I'_in_I2 in H'. }
+        
+        clear Nexti_lsc Nexti_ls Nexti_pn2 Nexti_pn2'.
+
+        set Nx2' := <[p := next']> Nx2.
+        set I2' := intf_merge I I2.
+        set s2' := (FP2, C2, Ht2, Mk2, Nx2', Ky2, I2'): snapshot.
+        set M2' := <[T2 + 1 := s2']> M2.
+
+        assert (abs s2 = C2) as Habs2'.
+        { rewrite Hs2. by unfold abs. }
+        assert (dom I ⊆ dom I2) as Dom_I_in_I2.
+        { by apply Hflupd. }
+        iAssert (⌜snapshot_constraints s2'⌝)%I as "SShot2'".
+        { iPureIntro. exists FP2, C2, Ht2, Mk2, Nx2', Ky2, I2'.
+          repeat split; try done.
+          rewrite /Nx2'. rewrite dom_insert_L.
+          assert (p ∈ dom Nx2) as H'. 
+          { rewrite Hs2 in FP_p2. rewrite Dom_Nx2. by unfold FP in FP_p2. }
+          clear -H' Dom_Nx2. set_solver.
+          rewrite /I2'. rewrite intf_merge_dom; try done. }
+        
+        assert (FP s2' = FP s2) as FP_s2'.
+        { by rewrite Hs2 /s2'; unfold FP. }
+        assert (∀ n, n ≠ p → Next s2' n = Next s2 n) as HN.
+        { intros n Hnp. 
+          rewrite /Next /s2' Hs2 /= /Nx2' lookup_insert_ne; try done. }
+        assert (Next s2' p = <[0:=c]> (Next s2 p)) as HNp.
+        { by rewrite /s2' Hs2 /Next /Nx2' lookup_insert Def_next' /Next Hs2. }
+        assert (∀ n, Key s2' n = Key s2 n) as HK.
+        { by rewrite /Key /s2' Hs2 /=. }
+        assert (∀ n, Height s2' n = Height s2 n) as HT.
+        { by rewrite /s2' Hs2 /=. }
+        assert (∀ n, n ∈ dom I → FI s2' n = I !!! n) as HI.
+        { rewrite /FI /s2' /= /I2'. intros n Hn. 
+          rewrite intf_merge_lookup; try done. }
+        assert (∀ n, n ∈ dom I2 → n ∉ dom I → FI s2' n = FI s2 n) as HI'.
+        { rewrite /FI /s2' Hs2 /= /I2'. intros n Hn Hn'. 
+          rewrite intf_merge_lookup_ne; try done. clear -Hn Hn'; set_solver. }
+        assert (∀ n, Mark s2' n = Mark s2 n) as HM.
+        { by rewrite /FI /s2' Hs2. }
+        assert (FP s2 = dom I2) as FP_I2.
+        { by rewrite Hs2 /FP. }
+
+        assert (abs s2' = abs s2) as Habs'.
+        { by rewrite /abs /s2' Hs2. }
+        iAssert (dsRepI _ _ _ _ γ_r (abs s2'))%I with "[Ds]" as "Ds".
+        { by rewrite Habs'. }
+        iAssert (own γ_ks (● prodKS (KS, abs s2')))%I with "[GKS]" as "GKS".
+        { by rewrite Habs'. }
+        iAssert (resources _ _ γ_ks s2')%I 
+          with "[GKS Nodes_KS Node_p Nodes_rest]" as "Res".
+        { iFrame "GKS". rewrite FP_s2'. iSplitR "Nodes_KS".
+          rewrite (big_opS_delete _ (FP s2) p); try done.
+          iSplitL "Node_p". rewrite Def_next' HNp HM HK HT. done.
+          iApply (big_sepS_mono with "Nodes_rest"); try done.
+          intros x Hx. iIntros "Hn". rewrite HK HM HT HN. done.
+          clear -Hx; set_solver.
+          iApply (big_sepS_mono with "Nodes_KS"); try done.
+          intros x Hx. iIntros "Hn".
+          assert (Content s2' x = Content s2 x) as ->.
+          { rewrite /Content /Marki HM HK. done. }
+          assert (keyset (FI s2' x) = keyset (FI s2 x)) as ->.
+          { destruct (decide (x ∈ dom I)) as [Hx1 | Hx1].
+            rewrite HI; try done. destruct Hflupd as (_&_&_&_&_&_&_&_&H').
+            rewrite -I2_eq_s2 H'; try done.
+            rewrite HI'; try done. by rewrite -FP_I2. }
+          done. }
+        
+        iAssert (⌜∀ n k, n ∈ FP s2' → k ∈ keyset (FI s2' n) →
+          (k ∈ abs s2' ↔ k ∈ Content s2' n)⌝)%I as "%Hks".
+        { iDestruct "Res" as "(GKS & _ & HKS)".
+          iPoseProof (keyset_summary with "GKS HKS") as "%H'"; try done. }
+        
+        assert (p ∈ dom I) as p_in_I.
+        { destruct Hflupd as (->&_). clear; set_solver. }
+
+        assert (per_tick_inv hd tl s2') as PT_s2'.
+        { destruct PT_s2 as (PT1'&PT2'&PT3'&PT4'&PT5'&PT6'&PT7').
+          split; last split; last split; last split; last split; last split.
+          - rewrite FP_s2' !HK !HM !HT. repeat split; try apply PT1'. 
+            destruct (decide (p = hd)) as [-> | Hphd]. 
+            rewrite HNp. rewrite lookup_insert_ne. apply PT1'. 
+            clear -HL; lia.
+            all: rewrite HN; try done; apply PT1'.
+            - rewrite /GFI FP_s2'.
+              assert (([^op set] x ∈ FP s2, FI s2' x) 
+                = ([^op set] x ∈ FP s2, I2' !!! x)) as ->.
+              { apply big_opS_ext. intros x Hx'.
+                by rewrite /s2' /FI /=. }
+              unfold GFI in PT2'.
+              assert (([^op set] x ∈ FP s2, I2' !!! x) 
+                = ([^op set] x ∈ FP s2, FI s2 x)) as ->; last done.
+              rewrite {1 3}Hs2 /FP -Dom_I2.
+              assert (([^op set] x ∈ dom I2, FI s2 x) 
+                = ([^op set] x ∈ dom I2, I2 !!! x)) as ->.
+              { apply big_opS_ext. intros x Hx'.
+                by rewrite Hs2 /FI /=. }
+              symmetry. apply (intf_merge_intfEq I); try done.
+              assert (([^op set] x ∈ dom I, I2 !!! x)
+                = ([^op set] x ∈ dom I, FI s2 x)) as ->.
+              { apply big_opS_ext. intros x Hx.
+                rewrite Hs2; unfold FI; try done. }
+              by apply Hflupd.
+          - apply Hks. 
+          - intros n Hn. assert (Hnn := Hn). rewrite FP_s2' in Hn. apply PT4' in Hn.
+            destruct (decide (n ∈ dom I)) as [Hn' | Hn'].
+            + destruct (decide (n = p)) as [-> | Hnp].
+              * rewrite HNp HK HM HT HI; try done.
+                destruct Hn as (Hn1&Hn2&Hn3&Hn4&Hn5&Hn6).
+                split; last split; last split; last split; last split; try done.
+                intros H'. assert (H1' := H'). apply Hn2 in H1'. 
+                rewrite dom_insert_L H1'.
+                assert (0 ∈ gset_seq 0 (Height s2 p - 1)) as H''.
+                { rewrite elem_of_gset_seq; split; clear; lia. }
+                clear -H''; set_solver. 
+                rewrite lookup_insert. apply Hflupd.
+              * rewrite HM HT HK HI; try done. rewrite HN; try done.
+                destruct Hn as (Hn1&Hn2&Hn3&Hn4&Hn5&Hn6).
+                split; last split; last split; last split; last split; try done.
+                apply Hflupd. all: done.
+            + rewrite HK HM HT HN; try done. rewrite HI'; try done.
+              by rewrite FP_s2' FP_I2 in Hnn. clear -p_in_I Hn'; set_solver.
+          - intros n1 n2. destruct (decide (n1 = p)) as [-> | Hn1p].
+            + rewrite /Nexti HNp !HK.
+              rewrite lookup_insert. intros [=<-]. apply Hflupd.
+            + rewrite !HK /Nexti HN; try done. apply PT5'. 
+          - intros n1 n2 i'. rewrite FP_s2'. 
+            destruct (decide (n1 = p)) as [-> | Hn1p].
+            + rewrite /Nexti HNp. destruct (decide (i' = 0)) as [-> | Hi'i].
+              rewrite lookup_insert. intros [=<-]. done.
+              rewrite lookup_insert_ne; try done. apply PT6'.
+            + rewrite /Nexti HN; try done. apply PT6'.
+          - intros n1 n2 i. rewrite /Nexti. 
+            destruct (decide (n1 = p)) as [-> | Hn1p]; last first.
+            { rewrite HT HN; try done. apply PT7'. }
+            rewrite HNp. destruct (decide (i = 0)) as [-> | Hi0].
+            + rewrite lookup_insert HT. intros [=<-]. apply PT4' in FP_c2.
+              destruct FP_c2 as (_&_&_&H'&_). apply Ht_c2.
+            + rewrite HT lookup_insert_ne; try done. apply PT7'. }
+        assert (transition_inv s2 s2') as Trans_s2.
+        { repeat split; try rewrite FP_s2'; try done; last first.
+          - intros n i' Hfp. rewrite /Marki HM. done.
+          - intros n. rewrite /Marki HM. intros H' H''. 
+            rewrite H' in H''; try done. 
+          - intros n' i' Hn'. destruct (decide (n' = p)) as [-> | Hnp].
+            + rewrite /Marki HM /Nexti HNp. 
+              destruct (decide (i' = 0)) as [-> | Hi].
+              rewrite Mark_p2. clear; try done.
+              rewrite lookup_insert_ne; try done.
+            + rewrite /Marki /Nexti HM HN; try done. }
+        
+        iAssert (⌜dom M2 = gset_seq 0 T2⌝)%I as %Dom_M2. 
+        { by iDestruct "Hist" as (M2'') "(_&_&%&_)". }
+
+        iAssert (|==> hist _ _ _ _ γ_t γ_m M2' (T2+1))%I with "[Hist]" as ">Hist".
+        { iPoseProof (hist_upd _ _ _ _ _ _ _ _ _ s2' with "[%] [%] [$Hist]") as ">H'".
+          apply  Habs2. intros <-. rewrite map_eq_iff in HNp.
+          pose proof HNp 0 as HNp. rewrite Next_p2 lookup_insert in HNp.
+          inversion HNp; try done. by rewrite /M2'. }
+        iAssert (|={⊤ ∖ ∅ ∖ ↑cntrN N}=> 
+          helping_inv _ _ _ _ N γ_t γ_r γ_mt γ_msy M2' ∗ dsRep _ _ _ _ γ_r (abs s2'))%I with
+          "[Help Ds]" as ">(Help & Ds)".
+        { iMod (fupd_mask_subseteq (⊤ ∖ ↑cntrN N)) as "H'". { clear; set_solver. }
+          iPoseProof ("Upd" with "[%] [Ds] [Help]") as ">Help"; try done.
+          apply leibniz_equiv in Habs2. iMod "H'" as "_". by iModIntro. }
+        iPoseProof (snapshot_current with "[%] [#] [$Hist]") 
+          as ">(#Past_s2'&Hist)"; try done.
+        iEval (rewrite /M2' lookup_total_insert) in "Past_s2'".
+
+        iAssert (traversal_inv _ _ _ _ γ_m t0 0 k p c)%I as "#Htr'".
+        { iSplitL; iExists s2'; iFrame "Past_s2'". iPureIntro. 
+          repeat split; try (by rewrite FP_s2' || done).
+          by rewrite HK. rewrite /Marki HM Mark_p2. done. rewrite HT. done.
+          by rewrite /Nexti HNp lookup_insert. iPureIntro. split. 
+          by rewrite FP_s2'. by rewrite HT. }
+        iAssert (⌜Marki s2 c 0 = false⌝ -∗ ⌜Key s1 c = k⌝ -∗
+          ∃ s : snapshot, past_state Σ Hg1 Hg2 Hg3 γ_m t0 s ∗
+            ⌜k ∈ abs s ∧ k = Key s c ∧ c ∈ FP s ∧ Marki s c 0 = false⌝)%I as "#Hcase1".
+        { iIntros "%Marki_c2 %Key_c2". rewrite -Key_c21 in Key_c2.
+          iExists s2'. iFrame "Past_s2'". iPureIntro. rewrite -FP_s2' in FP_c2.
+          assert (Marki s2' c 0 = false) as Marki_c2'.
+          { rewrite /Marki HM. apply Marki_c2. }
+          repeat split; try done.
+          pose proof Hks c k FP_c2 as Hks. apply Hks. 
+          apply (in_keyset hd tl s2' p c k); try done.
+          rewrite FP_s2'. done. rewrite /Marki HM. done.
+          rewrite /Nexti HNp lookup_insert. done. rewrite !HK. 
+          clear -Key_c2 Key_pk; lia.
+          rewrite /Content Marki_c2' HK Key_c2. clear; set_solver. 
+          by rewrite HK. }
+        iAssert (⌜Marki s2 c 0 = false⌝ -∗ ⌜k < Key s1 c⌝ -∗
+          ∃ s : snapshot, past_state Σ Hg1 Hg2 Hg3 γ_m t0 s ∗
+            ⌜(k ∉ abs s) ∧ k < Key s c ∧ c ∈ FP s⌝)%I as "#Hcase2".
+        { iIntros "%Marki_c2 %Key_c2". rewrite -Key_c21 in Key_c2.
+          iExists s2'. iFrame "Past_s2'". iPureIntro. rewrite -FP_s2' in FP_c2.
+          assert (Marki s2' c 0 = false) as Marki_c2'.
+          { rewrite /Marki HM. apply Marki_c2. }
+          repeat split; try done.
+          assert (k ∈ keyset (FI s2' c)) as KS_k.
+          { apply (in_keyset hd tl s2' p c k); try done.
+            rewrite FP_s2'. done. rewrite /Marki HM. done.
+            rewrite /Nexti HNp lookup_insert. done. rewrite !HK. 
+            clear -Key_c2 Key_pk; lia. }
+          pose proof Hks c k FP_c2 KS_k as Hks. intros H'%Hks. 
+          rewrite /Content Marki_c2' HK elem_of_singleton in H'. 
+          clear -Key_c2 H'; lia. by rewrite HK. }
+  
+
+        iModIntro. iSplitR "Hpost".
+        { iNext. iExists M2', (T2+1), s2'. iFrame "∗#%". 
+          iSplitR. iPureIntro. rewrite /M2'. by rewrite lookup_total_insert.
+          iExists hd, tl. iFrame "∗#%".
+          iPureIntro; rewrite /M2'; split.
+          - intros t Ht. destruct (decide (t = T2+1)) as [-> | Ht'].
+            + by rewrite lookup_total_insert.
+            + rewrite lookup_total_insert_ne; try done. apply PT2.
+              clear -Ht' Ht; lia.
+          - intros t Ht. destruct (decide (t = T2)) as [-> | Ht'].
+            + rewrite lookup_total_insert. rewrite lookup_total_insert_ne.
+              apply leibniz_equiv in Habs2. by rewrite Habs2. clear; lia.
+            + rewrite !lookup_total_insert_ne. apply Trans_M2.
+              all: clear -Ht Ht'; lia. }
+        wp_pures.
+
+        awp_apply findNext_spec.
+        iInv "HInv" as (M3 T3 s3) "(>Ds & >%Habs3 & >Hist & Help & >Templ)".
+        iDestruct "Templ" as (hd' tl')"(HR & SShot3 & Res & %PT3 & %Trans_M3)".
+        iAssert (⌜hd' = hd ∧ tl' = tl⌝)%I as %[-> ->]. admit.
+        iDestruct "Res" as "(GKS & Nodes & Nodes_KS)".
+        iAssert (⌜c ∈ FP s3⌝)%I as %FP_c3.
+        { apply leibniz_equiv in Habs3. rewrite -Habs3.
+          iDestruct "FP_c" as (s)"(Past_s & %FP_c & %Ht_c)".
+          iApply (in_FP_2 with "[%] [$Hist] [$Past_s] [%]"); try done. }
+        rewrite (big_sepS_delete _ (FP s3) c); last by eauto.
+        iDestruct "Nodes" as "(Node_c & Nodes_rest)".
+        iAssert (⌜0 < Height s3 c⌝)%I as %Height_c3.
+        { apply leibniz_equiv in Habs3. rewrite -Habs3.
+          iDestruct "FP_c" as (s)"(Past_s & %FP_c & %Ht_c)".
+          iPoseProof (height_eq_2 Σ Hg1 Hg2 Hg3 c with "[%] [$] [$Past_s] [%]") as "->"; 
+            try done. }
+        iAssert ((node Σ c (Height s3 c) (Mark s3 c) (Next s3 c) (Key s3 c)) 
+          ∗ ⌜0 < Height s3 c⌝)%I with "[Node_c]" as "Hpre".
+        { iFrame "Node_c %". }
+        iAaccIntro with "Hpre".
+        { iIntros "(Node_c & _)". iModIntro. iFrame "Hpost".
+          iNext; iExists M3, T3, s3. iFrame "∗%#". iExists hd, tl. iFrame "∗%#". 
+          rewrite (big_sepS_delete _ (FP s3) c); last by eauto. 
+          iFrame "Nodes_rest". iFrame. }
+        iIntros (m' cn') "(Node_c & %Mark_c3 & %Next_c3)".
+        iAssert (⌜per_tick_inv hd tl s3⌝)%I as %PT_s3.
+        { iApply (per_tick_current with "[%] [%] [$Hist]"); try done. }
+        iAssert (⌜m' = false⌝ -∗ ⌜Marki s2 c 0 = false⌝)%I as %Marki_c2.
+        { iIntros "%". subst m'. destruct (decide (Marki s2 c 0 = false)); try done.
+          iExFalso. rewrite not_false_iff_true in n.
+          iAssert (⌜Marki s3 c 0 = Marki s2 c 0⌝)%I as %H'.
+          { apply leibniz_equiv in Habs3. rewrite -Habs3.
+            iPoseProof (marking_mono_2 _ _ _ _ c with "[%] [$Hist] [$Past_s2] [%]") 
+              as "->"; try done. }
+          rewrite n /Marki H in H'. exfalso; clear -H'; done. }
+    
+        iModIntro. iSplitR "Hpost".
+        { iNext. iExists M3, T3, s3. iFrame "∗%". iExists hd, tl. iFrame "∗%".
+          rewrite (big_sepS_delete _ (FP s3) c); last by eauto.
+          iFrame "Nodes_rest". iFrame. }
+        destruct m'; wp_pures.
+        { iApply ("Hpost" $! None). done. }
+        assert (Marki s2 c 0 = false) as H'.
+        { by apply Marki_c2. }
+        destruct (bool_decide (#res = #1)) eqn: Hbool1.
+        { wp_pures. iApply ("Hpost" $! (Some (p, c, true))). iSimpl.
+          iFrame "Htr'". iModIntro. iIntros "_". iApply "Hcase1"; try done.
+          iPureIntro. rewrite bool_decide_eq_true in Hbool1. inversion Hbool1.
+          rewrite decide_False in Hif. rewrite decide_True in Hif. done.
+          clear -H0; lia. intros ->. clear -H0; lia. }
+        { wp_pures. iApply ("Hpost" $! (Some (p, c, false))). iSimpl.
+          iFrame "Htr'". iModIntro. iIntros "_". iApply "Hcase2"; try done.
+          iPureIntro. rewrite bool_decide_eq_false in Hbool1.
+          rewrite decide_False in Hif; try done. rewrite decide_False in Hif. done.
+          intros ->. apply Hbool1; clear; apply f_equal; apply f_equal; lia. }
+      + iDestruct "SShot2" as %[FP2 [C2 [Ht2 [Mk2 [Nx2 [Ky2 [I2 
+          [Hs2 [Dom_Ht2 [Dom_Mk2 [Dom_Nx2 [Dom_Ky2 Dom_I2]]]]]]]]]]]].
+        set Nx2' := <[p := next']> Nx2.
+        set s2' := (FP2, C2, Ht2, Mk2, Nx2', Ky2, I2): snapshot.
+        set M2' := <[T2 + 1 := s2']> M2.
+        
+        assert (FP s2' = FP s2) as FP_s2'.
+        { by rewrite /FP /s2' Hs2. }
+        assert (abs s2' = abs s2) as Habs'.
+        { by rewrite /abs /s2' Hs2. }
+        iAssert (dsRepI _ _ _ _ γ_r (abs s2'))%I with "[Ds]" as "Ds".
+        { by rewrite Habs'. }
+        iAssert (own γ_ks (● prodKS (KS, abs s2')))%I with "[GKS]" as "GKS".
+        { by rewrite Habs'. }
+        assert (∀ n, n ≠ p → Next s2' n = Next s2 n) as HN.
+        { intros n Hnc. 
+          rewrite /Next /s2' Hs2 /= /Nx2' lookup_insert_ne; try done. }
+        assert (Next s2' p = <[i:=c]> (Next s2 p)) as HNp.
+        { by rewrite /s2' Hs2 /Next /Nx2' lookup_insert Def_next' /Next Hs2. }
+        assert (∀ n, Key s2' n = Key s2 n) as HK.
+        { by rewrite /Key /s2' Hs2 /=. }
+        assert (∀ n, FI s2' n = FI s2 n) as HI.
+        { by rewrite /FI /s2' Hs2 /=. }
+        assert (∀ n, Mark s2' n = Mark s2 n) as HM.
+        { by rewrite /FI /s2' Hs2. }
+        assert (∀ n, Height s2' n = Height s2 n) as HT.
+        { by rewrite /FI /s2' Hs2. }
+        
+        iAssert (⌜snapshot_constraints s2'⌝)%I as "SShot2'".
+        { iPureIntro. exists FP2, C2, Ht2, Mk2, Nx2', Ky2, I2.
+          repeat split; try done.
+          rewrite /Nx2'. rewrite dom_insert_L.
+          assert (p ∈ dom Nx2). 
+          { rewrite Hs2 in FP_p2. rewrite Dom_Nx2. by unfold FP in FP_p2. }
+          clear -H Dom_Nx2. set_solver. }
+        
+        iAssert (resources _ _ γ_ks s2')%I 
+          with "[GKS Nodes_KS Node_p Nodes_rest]" as "Res".
+        { iFrame "GKS". rewrite FP_s2'. iSplitR "Nodes_KS".
+          rewrite (big_opS_delete _ (FP s2) p); try done.
+          iSplitL "Node_p". rewrite Def_next' HNp HT HM HK. done.
+          iApply (big_sepS_mono with "Nodes_rest"); try done.
+          intros x Hx. iIntros "Hn". rewrite HK HT HM HN. done.
+          clear -Hx; set_solver.
+          iApply (big_sepS_mono with "Nodes_KS"); try done.
+          intros x Hx. iIntros "Hn". rewrite HI.
+          assert (Content s2' x = Content s2 x) as ->.
+          rewrite /Content HK /Marki HM. done. done. }
+
+        assert (per_tick_inv hd tl s2') as PT_s2'.
+        { destruct PT_s2 as (PT1'&PT2'&PT3'&PT4'&PT5'&PT6'&PT7').
+          split; last split; last split; last split; last split; last split.
+          - rewrite FP_s2' !HK !HM !HT. repeat split; try apply PT1'. 
+            destruct (decide (p = hd)) as [-> | Hphd]. 
+            rewrite HNp. rewrite lookup_insert_ne; try done. apply PT1'.
+            clear -HiL; lia. all: rewrite HN; try done; apply PT1'.
+          - rewrite /s2' /GFI /FP /FI. by rewrite Hs2 /GFI /FP /FI in PT2'.
+          - intros n k'. rewrite FP_s2' HI Habs' /Content /Marki HM HK.
+            apply PT3'.
+          - intros n Hn. rewrite FP_s2' in Hn. apply PT4' in Hn.
+            destruct (decide (n = p)) as [-> | Hnp].
+            + rewrite HNp HK HI HT HM.
+              destruct Hn as (Hn1&Hn2&Hn3&Hn4&Hn5&Hn6).
+              split; last split; last split; last split; last split; try done.
+              * intros H'. assert (H1' := H'). apply Hn2 in H1'. 
+                rewrite dom_insert_L H1'.
+                assert (i ∈ gset_seq 0 (Height s2 p - 1)) as H''.
+                rewrite elem_of_gset_seq. split; try lia.
+                clear -H''; set_solver.
+              * rewrite lookup_insert_ne; try done.
+            + rewrite HK HT HI HM. rewrite HN; try done.
+          - intros n1 n2. destruct (decide (n1 = p)) as [-> | Hn1p].
+            + rewrite /Nexti HNp !HK. 
+              rewrite lookup_insert_ne; try done. apply PT5'.
+            + rewrite !HK /Nexti HN; try done. apply PT5'. 
+          - intros n1 n2 i'. rewrite FP_s2'. 
+            destruct (decide (n1 = p)) as [-> | Hn1p].
+            + rewrite /Nexti HNp. destruct (decide (i = i')) as [-> | Hi'i].
+              rewrite lookup_insert. intros [=<-]. done. 
+              rewrite lookup_insert_ne; try done. apply PT6'.
+            + rewrite /Nexti HN; try done. apply PT6'.
+          - intros n1 n2 i'. rewrite /Nexti. 
+            destruct (decide (n1 = p)) as [-> | Hn1p]; last first.
+            { rewrite HT HN; try done. apply PT7'. }
+            rewrite HNp. destruct (decide (i' = i)) as [-> | Hii'].
+            + rewrite lookup_insert HT. intros [=<-]. done.
+            + rewrite HT lookup_insert_ne; try done. apply PT7'. }
+        assert (transition_inv s2 s2') as Trans_s2.
+        { repeat split; try rewrite FP_s2'; try done; last first.
+          - intros n i' Hfp. rewrite /Marki HM. done.
+          - intros n. rewrite /Marki HM. intros H' H''. 
+            rewrite H' in H''; try done.
+          - intros n' i' Hn'. destruct (decide (n' = p)) as [-> | Hnp].
+            + rewrite /Marki HM /Nexti HNp. 
+              destruct (decide (i' = i)) as [-> | Hi].
+              rewrite Mark_p2. clear; try done.
+              rewrite lookup_insert_ne; try done.
+            + rewrite /Marki /Nexti HM HN; try done. }
+
+        iAssert (⌜dom M2 = gset_seq 0 T2⌝)%I as %Dom_M2. 
+        { by iDestruct "Hist" as (M2'') "(_&_&%&_)". }
+
+        iAssert (|==> hist _ _ _ _ γ_t γ_m M2' (T2+1))%I with "[Hist]" as ">Hist".
+        { iPoseProof (hist_upd _ _ _ _ _ _ _ _ _ s2' with "[%] [%] [$Hist]") as ">H'".
+          apply  Habs2. intros <-. rewrite map_eq_iff in HNp.
+          pose proof HNp i as HNp. rewrite Next_p2 lookup_insert in HNp.
+          inversion HNp; try done. by rewrite /M2'. }
+        iAssert (|={⊤ ∖ ∅ ∖ ↑cntrN N}=> 
+          helping_inv _ _ _ _ N γ_t γ_r γ_mt γ_msy M2' ∗ dsRep _ _ _ _ γ_r (abs s2'))%I with
+          "[Help Ds]" as ">(Help & Ds)".
+        { iMod (fupd_mask_subseteq (⊤ ∖ ↑cntrN N)) as "H'". { clear; set_solver. }
+          iPoseProof ("Upd" with "[%] [Ds] [Help]") as ">Help"; try done.
+          apply leibniz_equiv in Habs2. iMod "H'" as "_". by iModIntro. }
+        iPoseProof (snapshot_current with "[%] [#] [$Hist]") 
+          as ">(#Past_s2'&Hist)"; try done.
+        iEval (rewrite /M2' lookup_total_insert) in "Past_s2'".
+
+        iAssert (traversal_inv _ _ _ _ γ_m t0 i k p c)%I as "#Htr'".
+        { iSplitL; iExists s2'; iFrame "Past_s2'". iPureIntro. 
+          repeat split; try (by rewrite FP_s2' || done).
+          by rewrite HK. rewrite /Marki HM. apply PT_s2 in FP_p2.
+          destruct FP_p2 as (H'&_). apply H'. by exists i. rewrite HT. done.
+          iPureIntro. split. by rewrite FP_s2'. by rewrite HT. }
+
+        iModIntro. iSplitR "Hpost".
+        { iNext. iExists M2', (T2+1), s2'. iFrame "∗#%". 
+          iSplitR. iPureIntro. rewrite /M2'. by rewrite lookup_total_insert.
+          iExists hd, tl. iFrame "∗#%".
+          iPureIntro; rewrite /M2'; split.
+          - intros t Ht. destruct (decide (t = T2+1)) as [-> | Ht'].
+            + by rewrite lookup_total_insert.
+            + rewrite lookup_total_insert_ne; try done. apply PT2.
+              clear -Ht' Ht; lia.
+          - intros t Ht. destruct (decide (t = T2)) as [-> | Ht'].
+            + rewrite lookup_total_insert. rewrite lookup_total_insert_ne.
+              apply leibniz_equiv in Habs2. by rewrite Habs2. clear; lia.
+            + rewrite !lookup_total_insert_ne. apply Trans_M2.
+              all: clear -Ht Ht'; lia. }
+        wp_pures.
+          
+        awp_apply findNext_spec.
+        iInv "HInv" as (M3 T3 s3) "(>Ds & >%Habs3 & >Hist & Help & >Templ)".
+        iDestruct "Templ" as (hd' tl')"(HR & SShot3 & Res & %PT3 & %Trans_M3)".
+        iAssert (⌜hd' = hd ∧ tl' = tl⌝)%I as %[-> ->]. admit.
+        iDestruct "Res" as "(GKS & Nodes & Nodes_KS)".
+        iAssert (⌜c ∈ FP s3⌝)%I as %FP_c3.
+        { apply leibniz_equiv in Habs3. rewrite -Habs3.
+          iDestruct "FP_c" as (s)"(Past_s & %FP_c & %Ht_c)".
+          iApply (in_FP_2 with "[%] [$Hist] [$Past_s] [%]"); try done. }
+        rewrite (big_sepS_delete _ (FP s3) c); last by eauto.
+        iDestruct "Nodes" as "(Node_c & Nodes_rest)".
+        iAssert (⌜i < Height s3 c⌝)%I as %Height_c3.
+        { apply leibniz_equiv in Habs3. rewrite -Habs3.
+          iDestruct "FP_c" as (s)"(Past_s & %FP_c & %Ht_c)".
+          iPoseProof (height_eq_2 Σ Hg1 Hg2 Hg3 c with "[%] [$] [$Past_s] [%]") as "->"; 
+            try done. }
+        iAssert ((node Σ c (Height s3 c) (Mark s3 c) (Next s3 c) (Key s3 c)) 
+          ∗ ⌜i < Height s3 c⌝)%I with "[Node_c]" as "Hpre".
+        { iFrame "Node_c %". }
+        iAaccIntro with "Hpre".
+        { iIntros "(Node_c & _)". iModIntro. iFrame "Hpost".
+          iNext; iExists M3, T3, s3. iFrame "∗%#". iExists hd, tl. iFrame "∗%#". 
+          rewrite (big_sepS_delete _ (FP s3) c); last by eauto. 
+          iFrame "Nodes_rest". iFrame. }
+        iIntros (m' cn') "(Node_c & %Mark_c3 & %Next_c3)".
+        iAssert (⌜per_tick_inv hd tl s3⌝)%I as %PT_s3.
+        { iApply (per_tick_current with "[%] [%] [$Hist]"); try done. }
+    
+        iModIntro. iSplitR "Hpost".
+        { iNext. iExists M3, T3, s3. iFrame "∗%". iExists hd, tl. iFrame "∗%".
+          rewrite (big_sepS_delete _ (FP s3) c); last by eauto.
+          iFrame "Nodes_rest". iFrame. }
+        destruct m'; wp_pures.
+        { iApply ("Hpost" $! None). done. }
+        destruct (bool_decide (#res = #1)) eqn: Hbool1.
+        { wp_pures. iApply ("Hpost" $! (Some (p, c, true))). iSimpl.
+          iModIntro. iFrame "Htr'". iIntros "%H'". clear -Hi0 H'; lia. }
+        { wp_pures. iApply ("Hpost" $! (Some (p, c, false))). iSimpl.
+          iModIntro. iFrame "Htr'". iIntros "%H'". clear -Hi0 H'; lia. }
+  Admitted.
+
+  Lemma traverse_pop_spec Σ Hg1 Hg2 Hg3 N γ_t γ_r γ_m γ_mt γ_msy r tid t0 k 
+    preds succs ps0 ss0 (i: nat) hd tl:
+    main_inv Σ Hg1 Hg2 Hg3 N γ_t γ_r γ_m γ_mt γ_msy r -∗
+    thread_start Σ Hg1 Hg2 Hg3 γ_t γ_mt tid t0 -∗
+    □ update_helping_protocol Σ Hg1 Hg2 Hg3 N γ_t γ_r γ_mt γ_msy -∗ 
+    ⌜1 < L ∧ 0 < k < W⌝ -∗
+        {{{ is_array Σ Hg1 preds ps0 ∗ is_array Σ Hg1 succs ss0 
+            ∗ ⌜length ps0 = L⌝ ∗ ⌜length ss0 = L⌝ ∗ ⌜i+1 < L⌝
+            ∗ ⌜ps0 !!! (L-1) = hd⌝ ∗ ⌜ss0 !!! (L-1) = tl⌝
+            ∗ (∀ j, ⌜i < j < L⌝ → traversal_inv Σ Hg1 Hg2 Hg3 γ_m t0 j k (ps0 !!! j) (ss0 !!! j)) }}}
+          traverse_pop #k #preds #succs #i @ ⊤
+        {{{ (ores: option (loc * loc * bool)) (ps ss: list Node) (b: bool), 
+              RET (match ores with 
+                    None => NONEV 
+                  | Some res => SOMEV (#res.1.1,#res.1.2,#res.2) end);
+              match ores with 
+                None => is_array Σ Hg1 preds ps0 ∗ is_array Σ Hg1 succs ss0
+              | Some res => 
+                ⌜res.1.1 = preds⌝ ∗ ⌜res.1.2 = succs⌝ ∗ ⌜res.2 = b⌝
+              ∗ is_array Σ Hg1 preds ps ∗ is_array Σ Hg1 succs ss
+              ∗ ⌜length ps = L⌝ ∗ ⌜length ss = L⌝
+              ∗ ⌜ps !!! (L-1) = hd⌝ ∗ ⌜ss !!! (L-1) = tl⌝
+              ∗ (∀ j, ⌜i-1 < j < L⌝ → traversal_inv Σ Hg1 Hg2 Hg3 γ_m t0 j k (ps !!! j) (ss !!! j))
+              ∗ (⌜i = 0⌝ →  let p := ps !!! 0 in
+                            let c := ss !!! 0 in
+                            traversal_inv Σ Hg1 Hg2 Hg3 γ_m t0 0 k p c ∗ 
+                            (∃ s, past_state Σ Hg1 Hg2 Hg3 γ_m t0 s ∗
+                              ⌜if b then 
+                                  k ∈ abs s ∧ k = Key s c 
+                                  ∧ c ∈ FP s ∧ Marki s c 0 = false
+                                else 
+                                  k ∉ abs s ∧ k < Key s c 
+                                  ∧ c ∈ FP s⌝)) end }}}.
+  Proof.
+    iIntros "#HInv #Thd_st #Upd [%HL %Range_k]". iIntros (Φ) "!# Hpre Hpost".
+    iDestruct "Hpre" as "(Hpreds & Hsuccs & %Len_ps0 & %Len_ss0 & %Len_i 
+      & %Hps0_L & %Hss0_L & #Hj)". 
+    wp_lam. wp_pures. iEval (rewrite /is_array) in "Hpreds".
+    assert (is_Some (ps0 !! (i+1))) as [p Hp].
+    { by rewrite lookup_lt_is_Some Len_ps0. } 
+    assert (Z.of_nat (i+1) = (Z.of_nat i + 1)%Z) as H' by lia.
+    iEval (rewrite <-H'). clear H'.
+    wp_apply (wp_load_offset _ _ _ (DfracOwn 1) (i+1) ((λ n : loc, #n) <$> ps0) #p
+      with "[Hpreds]"); try done. 
+    { by rewrite list_lookup_fmap Hp /=. }
+    iIntros "Hpreds".
+    iAssert (is_array Σ Hg1 preds ps0) with "[Hpreds]" as "Hpreds".
+    { unfold is_array. iFrame. }
+    wp_pures. wp_bind (findNext _ _)%E. 
+    awp_apply findNext_spec.
+    iInv "HInv" as (M0 T0 s0) "(>Ds & >%Habs0 & >Hist & Help & >Templ)".
+    iDestruct "Templ" as (hd' tl') "(HR & SShot0 & Res & %PT0 & %Trans_M0)".
+    iAssert (⌜hd' = hd ∧ tl' = tl⌝)%I as %[-> ->]. admit.
+    iDestruct "Res" as "(GKS & Nodes & Nodes_KS)".
+    iAssert (traversal_inv Σ Hg1 Hg2 Hg3 γ_m t0 (i+1) k p (ss0 !!! (i+1)%nat))%I as "#Htr_i1". 
+    { iAssert (⌜i < i+1 < L⌝)%I as "H'". by iPureIntro; lia.
+      iPoseProof ("Hj" with "H'") as "H''". 
+      apply list_lookup_total_correct in Hp. rewrite Hp. done. }
+    iAssert (⌜p ∈ FP s0⌝)%I as %FP_p0.
+    { apply leibniz_equiv in Habs0. rewrite -Habs0. 
+      iDestruct "Htr_i1" as "(H'&_)". iDestruct "H'" as (s)"(Past_s & %Htr_sp)".
+      destruct Htr_sp as (H'&_).
+      iApply (in_FP_2 with "[%] [$Hist] [$Past_s] [%]"); try done. }
+    rewrite (big_sepS_delete _ (FP s0) p); last by eauto.
+    iDestruct "Nodes" as "(Node_p & Nodes_rest)".
+    iAssert (⌜i < Height s0 p⌝)%I as %Height_p0.
+    { apply leibniz_equiv in Habs0. rewrite -Habs0.
+      iDestruct "Htr_i1" as "(H'&_)". iDestruct "H'" as (s)"(Past_s & %Htr_sp)".
+      destruct Htr_sp as (H''&_&_&H').
+      iPoseProof (height_eq_2 _ _ _ _ p with "[%] [$Hist] [$Past_s] [%]") as "->"; 
+        try done. iPureIntro. clear -H'; lia. }
+    iAssert ((node Σ p (Height s0 p) (Mark s0 p) (Next s0 p) (Key s0 p)) 
+      ∗ ⌜i < Height s0 p⌝)%I with "[Hj Node_p]" as "Hpre".
+    { iFrame "Node_p %". }
+    iAaccIntro with "Hpre".    
+    { iIntros "(Node_p&_)". iModIntro. iFrame "Hpost Hpreds Hsuccs".
+      iNext; iExists M0, T0, s0. iFrame "∗%#". iExists hd, tl. iFrame "∗%#". 
+      rewrite (big_sepS_delete _ (FP s0) p); last by eauto. iFrame. }
+    iIntros (m c) "(Node_p & %Mark_p0 & %Next_p0)".
+    iAssert (⌜per_tick_inv hd tl s0⌝)%I as %PT_s0.
+    { iApply (per_tick_current with "[%] [%] [$Hist]"); try done. }
+    iDestruct "Htr_i1" as "(Htr_p & Htr_si1)".
+    iDestruct "Htr_p" as (s)"(#Past_s & %Htr_p)".
+    iAssert (⌜Key s0 p = Key s p⌝)%I as %Key_p.
+    { apply leibniz_equiv in Habs0. rewrite -Habs0.
+      iPoseProof (key_eq_2 with "[%] [$Hist] [$Past_s] [%]") as "->"; try done.
+      apply Htr_p. }
+    iPoseProof (snapshot_current with "[%] [#] [$Hist]") 
+      as ">(#Past_s0&Hist)"; try done.
+    iAssert (|={⊤ ∖ ∅ ∖ ↑cntrN N}=> traversal_inv Σ Hg1 Hg2 Hg3 γ_m t0 i k p c ∗ 
+      hist Σ Hg1 Hg2 Hg3 γ_t γ_m M0 T0)%I with "[Hist]" as ">(#Hcase & Hist)".
+    { assert (Next s0 p !! i = Some c) as Next_p0'.
+      { rewrite lookup_lookup_total. by rewrite Next_p0. rewrite -elem_of_dom.
+        apply PT_s0 in FP_p0. destruct FP_p0 as (_&H'&_). rewrite H'.
+        rewrite elem_of_gset_seq. lia. intros ->. destruct PT_s0 as ((_&_&H''&_)&_).
+        destruct Htr_p as (_&H1'&_). clear -H1' Key_p H'' Range_k. lia. }
+      iAssert (∃ s1 : snapshot, past_state Σ Hg1 Hg2 Hg3 γ_m t0 s1 ∗ 
+        ⌜c ∈ FP s1 ∧ i < Height s1 c⌝)%I as "#Htr_c".
+      { iExists s0. iFrame "Past_s0". iPureIntro. 
+        destruct PT_s0 as (_&_&_&_&_&H'&H''). split. 
+        apply (H' p c i); try done. apply (H'' p c i); try done. }
+      iFrame "Htr_c". 
+      destruct (decide (i = 0)) as [-> | Hi0].
+      - destruct m.
+        + iAssert (⌜dom M0 = gset_seq 0 T0⌝)%I as %Dom_M0. 
+          { by iDestruct "Hist" as (M0'') "(_&_&%&_)". }
+          destruct Htr_p as (FP_ps&Key_ps&Mark_ps&Height_ps&_).
+          iDestruct "Past_s" as (ts)"(%t0_le_ts&Hts)".
+          iPoseProof (marking_witness with "[%] [Hist] [Hts] [%] [%] [%]") 
+            as "%HM"; try done. 
+          apply leibniz_equiv in Habs0. by rewrite /Marki Habs0.
+          destruct HM as [t [Ht [Hmt Hmt']]].
+          assert (0 ≤ t < T0) as Ht'. lia.
+          apply Trans_M0 in Ht'. rewrite Nat.add_1_r in Ht'.
+          destruct Ht' as (Hm'&_&_&_&_&Hfp'). 
+          assert (t ∈ dom M0) as t_in_M0. 
+          { rewrite Dom_M0 elem_of_gset_seq; lia. }
+          assert (H'' := t_in_M0).
+          apply elem_of_dom in t_in_M0. destruct t_in_M0 as [s' Hs'].
+          iPoseProof (snapshot_create Σ Hg1 Hg2 Hg3 t t0 with "[%] [$Hist]")
+            as ">(#Past_t & Hist)"; try done. lia.
+
+          iAssert (|={⊤ ∖ ∅ ∖ ↑cntrN N}=> own γ_m (◯ {[t := to_agree s']}) 
+            ∗ hist Σ Hg1 Hg2 Hg3 γ_t γ_m M0 T0)%I with "[Hist]" as ">(#Ht & Hist)".
+          { iDestruct "Hist" as (M')"(HT&HM'&%Dom_M&%M_eq&%M_neq)".
+            iPoseProof (own_update _ (● M') (● M' ⋅ ◯ {[t := to_agree s']}) 
+              with "HM'") as ">(HM' & #Ht')". 
+            { apply auth_update_alloc, local_update_unital_discrete. 
+              intros z Hm Hz. split; try done. rewrite left_id in Hz. 
+              rewrite -Hz. apply map_equiv_iff. intros x. apply M_eq in Hs'.
+              destruct (decide (x = t)) as [-> | Hxz].
+              - rewrite lookup_op Hs' lookup_insert. rewrite /op /cmra_op /=.
+                by rewrite agree_idemp.
+              - rewrite lookup_op lookup_insert_ne; try done. rewrite lookup_empty.
+                rewrite /op /cmra_op /=. destruct (M' !! x) eqn:H1'; 
+                rewrite H1'; try done. }
+            iModIntro. iFrame "Ht'". iExists M'. iFrame "∗%". } 
+          assert (ts ≤ t ≤ T0) as Ht' by lia.
+          iPoseProof (in_FP Σ Hg1 Hg2 Hg3 p with "[%] [$Hist] [$Hts] [%] [%]") 
+            as "%FP_pt"; try done.
+          pose proof Hm' p 0 FP_pt Hmt' as Hn'.
+
+          assert (S t ∈ dom M0) as Hst.
+          { rewrite Dom_M0 elem_of_gset_seq. lia. }
+          assert (t0 ≤ S t) as Hst' by lia.
+          iPoseProof (snapshot_create Σ Hg1 Hg2 Hg3 (S t) t0 with "[%] [$Hist]")
+            as ">(#Past_st & Hist)"; try done. lia. 
+          assert (FP_pst := FP_pt). apply Hfp' in FP_pst.
+          iPoseProof (next_unchanged with "[%] [$Hist] [$Past_st] [%] [%]")
+            as "%H'"; try done. rewrite -H' in Hn'.
+          apply leibniz_equiv in Habs0. rewrite Habs0 /Nexti Next_p0' in Hn'.
+          iPoseProof (height_eq with "[%] [$Hist] [$Hts] [%] [%]")
+            as "%HH"; try done.
+          iPoseProof (key_eq with "[%] [$Hist] [$Hts] [%] [%]")
+            as "%HK"; try done.
+          iModIntro. iFrame. iExists (M0 !!! t). iFrame "#". iPureIntro.
+          repeat split; try done. clear -HK Key_ps; lia.  clear -HH Height_ps; lia.
+        + iModIntro. iFrame.
+          iExists s0. iFrame "Past_s0". iPureIntro. 
+          repeat split; try done. destruct Htr_p as (_&H'&_). 
+          clear -H' Key_p; lia.
+      - iModIntro. iFrame.
+        iExists s. iFrame "Past_s". iPureIntro. repeat split; try apply Htr_p.
+        destruct Htr_p as (_&_&_&H'&_). clear -H'; lia. intros ?; try done. }
+    
+    iModIntro. iSplitR "Hpreds Hsuccs Hpost Hj".
+    { iNext. iExists M0, T0, s0. iFrame "∗%". iExists hd, tl. iFrame "∗%".
+      rewrite (big_sepS_delete _ (FP s0) p); last by eauto. iFrame. }
+    wp_pures. wp_apply (traverse_i_spec _ _ _ _ []); try done. 
+    { iPureIntro. lia. }
+    { iFrame "Hcase". iDestruct "Hcase" as "(_&H')". iFrame "H'". by iIntros "%". }
+
+    iIntros (ores) "Hores".
+    destruct ores as [[[p' c'] b]|]; last first.
+    { wp_pures. iSpecialize ("Hpost" $! None ps0 ss0 true). iApply "Hpost".
+      iFrame. done. }
+    iSimpl in "Hores". wp_pures. wp_bind (_ <- _)%E. 
+    iApply (array_store with "[Hpreds]").
+    { iFrame "Hpreds". iPureIntro. rewrite Len_ps0. lia. }
+    iIntros "!> Hpreds". wp_pures. wp_bind (_ <- _)%E. 
+    iApply (array_store with "[Hsuccs]").
+    { iFrame "Hsuccs". iPureIntro. rewrite Len_ss0. lia. }
+    iIntros "!> Hsuccs". wp_pures.
+    iSpecialize ("Hpost" $! (Some (preds,succs,b)) _ _ b).
+    iSimpl in "Hpost". iApply "Hpost".
+    iModIntro. iFrame "Hpreds Hsuccs". repeat (iSplitR; first by iPureIntro).
+    iDestruct "Hores" as "(#Htr & #Hzero)".
+    iSplitR. iPureIntro. by rewrite insert_length.
+    iSplitR. iPureIntro. by rewrite insert_length.
+    iSplitR. iPureIntro. rewrite list_lookup_total_insert_ne; try done. 
+    clear -Len_i; lia.  
+    iSplitR. iPureIntro. rewrite list_lookup_total_insert_ne; try done. 
+    clear -Len_i; lia.  
+    iSplitR. iIntros (j)"%Hj". destruct (decide (j = i)) as [-> | Hij].
+    { rewrite !list_lookup_total_insert. iFrame "#". 
+      all: try rewrite Len_ps0 Len_ss0; lia. }
+    iAssert (⌜i < j < L⌝)%I as "Hj'". { iPureIntro. lia. }
+    iPoseProof ("Hj" with "Hj'") as "H'".
+    rewrite !list_lookup_total_insert_ne; try done.
+    iIntros "%". subst i. rewrite !list_lookup_total_insert.
+    iFrame "∗#". iApply "Hzero". by iPureIntro.
+    all: try rewrite Len_ps0 Len_ss0; lia.
+  Admitted.
+
+  Lemma traverse_rec_spec Σ Hg1 Hg2 Hg3 N γ_t γ_r γ_m γ_mt γ_msy r tid 
+    t0 k preds succs ps0 ss0 (i: nat) hd tl:
+    main_inv Σ Hg1 Hg2 Hg3 N γ_t γ_r γ_m γ_mt γ_msy r -∗
+    thread_start Σ Hg1 Hg2 Hg3 γ_t γ_mt tid t0 -∗
+    □ update_helping_protocol Σ Hg1 Hg2 Hg3 N γ_t γ_r γ_mt γ_msy -∗ 
+    ⌜1 < L ∧ 0 < k < W⌝ -∗
+      {{{ is_array Σ Hg1 preds ps0 ∗ is_array Σ Hg1 succs ss0
+          ∗ ⌜length ps0 = L⌝ ∗ ⌜length ss0 = L⌝ ∗ ⌜i+1 < L⌝
+          ∗ ⌜ps0 !!! (L-1) = hd⌝ ∗ ⌜ss0 !!! (L-1) = tl⌝
+          ∗ (∀ j, ⌜i < j < L⌝ → traversal_inv Σ Hg1 Hg2 Hg3 γ_m t0 j k (ps0 !!! j) (ss0 !!! j)) }}}
+        traverse_rec #k #preds #succs #i @ ⊤
+      {{{ (ps ss: list Node) (res: bool), 
+            RET (#preds, #succs, #res);
+            is_array Σ Hg1 preds ps ∗ is_array Σ Hg1 succs ss
+          ∗ ⌜length ps = L⌝ ∗ ⌜length ss = L⌝
+          ∗ ⌜ps !!! (L-1) = hd⌝ ∗ ⌜ss !!! (L-1) = tl⌝
+          ∗ (∀ i, ⌜i < L⌝ → traversal_inv Σ Hg1 Hg2 Hg3 γ_m t0 i k (ps !!! i) (ss !!! i))
+          ∗ (let c := ss !!! 0 in 
+                ∃ s, past_state Σ Hg1 Hg2 Hg3 γ_m t0 s ∗
+                    ⌜if res then 
+                      k ∈ abs s ∧ k = Key s c ∧ c ∈ FP s ∧ Marki s c 0 = false
+                    else 
+                      k ∉ abs s ∧ k < Key s c ∧ c ∈ FP s⌝) }}}.
+  Proof.
+    iIntros "#HInv #Thd_st #Upd [%HL %Range_k]". iLöb as "IH" forall (i ps0 ss0). 
+    iIntros (Φ) "!# Hpre Hpost".
+    iDestruct "Hpre" as "(Hpreds & Hsuccs & %Len_ps0 & %Len_ss0 & %Len_i 
+      & %Hps0_L & %Hss0_L & #Hj)".
+    wp_lam. wp_pures. iApply fupd_wp.
+    iInv "HInv" as (M0 T0 s0) "(>Ds & >%Habs0 & >Hist & Help & >Templ)".
+    iDestruct "Templ" as (hd' tl')"(HR & SShot0 & Res & %PT0 & %Trans_M0)".
+    iAssert (⌜hd' = hd ∧ tl' = tl⌝)%I as %[-> ->]. admit.
+    iAssert (⌜per_tick_inv hd tl s0⌝)%I as %PT_s0.
+    { iApply (per_tick_current with "[%] [%] [$Hist]"); try done. }
+    iPoseProof (traversal_inv_hd_tl with "[%] [%] [%] [%] [#] [Hist]") 
+      as ">(#HtrL & Hist)"; try done.
+    iModIntro. iSplitR "Hpreds Hsuccs Hpost".
+    { iNext. iExists M0, T0, s0. iFrame "∗%". iExists hd, tl. iFrame "∗%". }
+    iModIntro.      
+    wp_apply (traverse_pop_spec with "[] [] [] [] [Hpreds Hsuccs]"); try done.
+    iFrame "Hpreds Hsuccs Hj %". iIntros (ores ps ss b)"Hores".
+    destruct ores as [[[preds' succs'] res] |]; last first.
+    { wp_pures. iDestruct "Hores" as "(Hpreds & Hsuccs)".
+      iApply ("IH" with "[Hpreds Hsuccs]"); try iFrame "∗%#". 
+      iSplitR. iPureIntro. lia. iIntros (j)"%Hj".
+      assert (j = L-1) as -> by lia. rewrite Hps0_L Hss0_L. iFrame "HtrL". }
+    wp_pures. iDestruct "Hores" as "(%H' & %H'' & %H1' & H1'')". 
+    rewrite /= in H' H'' H1'. subst preds' succs' b.  
+    iDestruct "H1''" as "(Hpreds & Hsuccs & %Len_ps & %Len_ss & %Hps_L 
+      & %Hss_L & #Hj' & #Hi0)".
+    destruct (bool_decide (#i = #0)) eqn: Hbool; wp_pures.
+    - rewrite bool_decide_eq_true in Hbool. inversion Hbool. iModIntro.
+      iApply "Hpost". iFrame "Hpreds Hsuccs %".
+      iAssert (⌜i = 0⌝)%I as "Htr0". { iPureIntro; lia. }
+      iDestruct ("Hi0" with "Htr0") as "#H'". iSplit.
+      + iIntros (j) "%Hj". destruct (decide (j = 0)) as [-> | Hj0].
+        * iDestruct "H'" as "(H' & _)". iFrame "H'".
+        * iApply "Hj'". iPureIntro; lia.
+      + iDestruct "H'" as "(_ & H')". iFrame "H'".
+    - iSpecialize ("IH" $! (i-1) ps ss).
+      rewrite bool_decide_eq_false in Hbool.
+      assert (i ≠ 0). { intros ->. apply Hbool. try done. }
+      assert (Z.sub i 1 = (i-1)%nat) as -> by lia.
+      iApply ("IH" with "[$Hpreds $Hsuccs]"); try done. iFrame "%#".
+      iPureIntro. clear -Len_i; lia.
+  Admitted.
+
+  Lemma traverse_spec (Σ : gFunctors) (H' : heapGS Σ) (H'' : dsG Σ) (H''' : hsG Σ)
+    N γ_t γ_r γ_m γ_mt γ_msy r tid t0 k (hd tl: Node):
+    main_inv Σ H' H'' H''' N γ_t γ_r γ_m γ_mt γ_msy r -∗
+    thread_start Σ H' H'' H''' γ_t γ_mt tid t0 -∗
+    □ update_helping_protocol Σ H' H'' H''' N γ_t γ_r γ_mt γ_msy -∗ 
+    ⌜1 < L ∧ 0 < k < W⌝ -∗
+      {{{ True }}}
+          traverse #hd #tl #k @ ⊤
+      {{{ (preds succs: loc) (ps ss: list Node) (res: bool), 
+            RET (#preds, #succs, #res);
+            (preds ↦∗ ((fun n => # (LitLoc n)) <$> ps))
+          ∗ (succs ↦∗ ((fun n => # (LitLoc n)) <$> ss))
+          ∗ ⌜length ps = L⌝ ∗ ⌜length ss = L⌝
+          ∗ ⌜ps !!! (L-1) = hd⌝ ∗ ⌜ss !!! (L-1) = tl⌝
+          ∗ (∀ i, ⌜i < L⌝ → traversal_inv Σ H' H'' H''' γ_m t0 i k (ps !!! i) (ss !!! i))
+          ∗ (let c := ss !!! 0 in 
+                ∃ s, past_state Σ H' H'' H''' γ_m t0 s ∗
+                    ⌜if res then 
+                      k ∈ abs s ∧ k = Key s c ∧ c ∈ FP s ∧ Marki s c 0 = false
+                    else 
+                      k ∉ abs s ∧ k < Key s c ∧ c ∈ FP s⌝) }}}.
+  Proof.
+    iIntros "#HInv #Thd_st #Upd [%HL %Range_k]". iIntros (Φ) "!# _ Hpost".
+    wp_lam. wp_pures. wp_bind (AllocN _ _)%E. 
+    iApply array_repeat. iPureIntro; lia.
+    iNext. iIntros (preds) "Hpreds".
+    wp_pures. wp_bind (AllocN _ _)%E.
+    iApply array_repeat. iPureIntro; lia.
+    iNext. iIntros (succs) "Hsuccs". wp_pures. iApply fupd_wp.
+    iInv "HInv" as (M0 T0 s0) "(>Ds & >%Habs0 & >Hist & Help & >Templ)".
+    iDestruct "Templ" as (hd' tl')"(HR & SShot0 & Res & %PT0 & %Trans_M0)".
+    iAssert (⌜hd' = hd ∧ tl' = tl⌝)%I as %[-> ->]. admit.
+    iAssert (⌜per_tick_inv hd tl s0⌝)%I as %PT_s0.
+    { iApply (per_tick_current with "[%] [%] [$Hist]"); try done. }
+    iPoseProof (traversal_inv_hd_tl with "[%] [%] [%] [%] [#] [Hist]") 
+      as ">(#HtrL & Hist)"; try done.
+    iModIntro. iSplitR "Hpreds Hsuccs Hpost".
+    { iNext. iExists M0, T0, s0. iFrame "∗%". iExists hd, tl. iFrame "∗%". }
+    iModIntro.      
+    wp_apply (traverse_rec_spec with "[] [] [] [] [Hpreds Hsuccs]"); try done.
+    iFrame "Hpreds Hsuccs".
+    iSplitR. iPureIntro. by rewrite replicate_length.
+    iSplitR. iPureIntro. by rewrite replicate_length.
+    iSplitR. iPureIntro. clear -HL; lia.
+    iSplitR. iPureIntro. rewrite lookup_total_replicate_2. done. lia.
+    iSplitR. iPureIntro. rewrite lookup_total_replicate_2. done. lia.
+    iIntros (j) "%Hj". 
+    assert (j = L-1) as -> by lia. rewrite !lookup_total_replicate_2.
+    all : try lia. iFrame "HtrL".
+  Admitted.
+  
+End HARRIS_SPEC.
