templates/lockfree/skiplist_insert.v
@@ -11,7 +11,7 @@ From iris.heap_lang.lib Require Import nondet_bool.
 From iris.bi.lib Require Import fractional.
 Set Default Proof Using "All".
 From iris.bi.lib Require Import fractional.
-Require Import list_flow_upd_insert.
+Require Import list_flow_upd_insert skiplist_util.
 Require Export skiplist_insert_maintenance.
 
   Lemma insertOp_spec (Σ : gFunctors) (Hg1 : heapGS Σ) (Hg2 : dsG Σ) (Hg3 : hsG Σ)
