templates/lockfree/traverse_module.v
@@ -1,0 +1,28 @@
+From iris.algebra Require Import excl auth cmra gmap agree gset numbers.
+From iris.algebra.lib Require Import dfrac_agree.
+From iris.heap_lang Require Export notation locations lang.
+From iris.base_logic.lib Require Export invariants.
+From iris.program_logic Require Export atomic.
+From iris.proofmode Require Import tactics.
+From iris.heap_lang Require Import proofmode par.
+From iris.bi.lib Require Import fractional.
+Set Default Proof Using "All".
+From iris.bi.lib Require Import fractional.
+From flows Require Import node_module.
+
+Parameter L : nat.
+
+Module Type TRAVERSE.
+  Declare Module NODE : NODE_IMPL.
+
+  Parameter traverse_rec : heap_lang.val.
+
+  Definition traverse : heap_lang.val :=
+    λ: "h" "t" "k",
+      let: "preds" := AllocN #L "h" in
+      let: "succs" := AllocN #L "t" in
+      traverse_rec "k" "preds" "succs" #(L-2)%nat.
+
+End TRAVERSE.
+
+
