templates/lockfree/traverse_spec_module.v
@@ -1,0 +1,118 @@
+From iris.algebra Require Import excl auth cmra gmap agree gset numbers.
+From iris.algebra.lib Require Import dfrac_agree.
+From iris.heap_lang Require Export notation locations lang.
+From iris.base_logic.lib Require Export invariants.
+From iris.program_logic Require Export atomic.
+From iris.proofmode Require Import tactics.
+From iris.heap_lang Require Import proofmode par.
+From iris.bi.lib Require Import fractional.
+From flows Require Import array_util skiplist_util.
+Set Default Proof Using "All".
+
+Module Type TRAVERSE_SPEC.
+  Declare Module TR : TRAVERSE.
+  Export TR.NODE SK DEFS.
+
+  Definition traversal_inv Σ Hg1 Hg2 Hg3 γ_m t0 i k p c : iProp Σ :=
+    (∃ s, past_state Σ Hg1 Hg2 Hg3 γ_m t0 s ∗ ⌜p ∈ FP s ∧ Key s p < k ∧ 
+      Marki s p 0 = false ∧ i < Height s p ∧ (i = 0 → Nexti s p i = Some c)⌝)
+  ∗ (∃ s, past_state Σ Hg1 Hg2 Hg3 γ_m t0 s ∗ ⌜c ∈ FP s ∧ i < Height s c⌝).
+
+  Lemma traversal_inv_hd_tl Σ Hg1 Hg2 Hg3 γ_m γ_t γ_mt hd tl M T s tid t0 k:
+    ⌜M !!! T ≡ s⌝ -∗ 
+    ⌜per_tick_inv hd tl s⌝ -∗
+    ⌜1 < L⌝ -∗
+    ⌜0 < k < W⌝ -∗
+    thread_start Σ Hg1 Hg2 Hg3 γ_t γ_mt tid t0 -∗
+    hist Σ Hg1 Hg2 Hg3 γ_t γ_m M T -∗
+      |==> traversal_inv Σ Hg1 Hg2 Hg3 γ_m t0 (L-1) k hd tl ∗ hist Σ Hg1 Hg2 Hg3 γ_t γ_m M T.
+  Proof.
+    iIntros "%Habs %PT %HL %Range_k #Thd_st Hist".
+    iPoseProof (snapshot_current with "[%] [#] [$]") 
+      as ">(#Past_s&Hist)"; try done.
+    destruct PT as ((H1'&H2'&H3'&H4'&H5'&H6'&H7'&H8'&H9')&_).
+    iModIntro. iFrame. iSplit; iExists s; iFrame "Past_s".
+    - iPureIntro; repeat split; try (done || lia).
+      set_solver. apply H4'. lia.
+    - iPureIntro; repeat split; try (done || lia). set_solver.
+  Qed. 
+
+  Parameter traverse_rec_spec : ∀ Σ Hg1 Hg2 Hg3 N γ_t γ_r γ_m γ_mt γ_msy r tid 
+    t0 k preds succs ps0 ss0 (i: nat) hd tl,
+    main_inv Σ Hg1 Hg2 Hg3 N γ_t γ_r γ_m γ_mt γ_msy r -∗
+    thread_start Σ Hg1 Hg2 Hg3 γ_t γ_mt tid t0 -∗
+    □ update_helping_protocol Σ Hg1 Hg2 Hg3 N γ_t γ_r γ_mt γ_msy -∗ 
+    ⌜1 < L ∧ 0 < k < W⌝ -∗
+      {{{ is_array Σ Hg1 preds ps0 ∗ is_array Σ Hg1 succs ss0
+          ∗ ⌜length ps0 = L⌝ ∗ ⌜length ss0 = L⌝ ∗ ⌜i+1 < L⌝
+          ∗ ⌜ps0 !!! (L-1) = hd⌝ ∗ ⌜ss0 !!! (L-1) = tl⌝
+          ∗ (∀ j, ⌜i < j < L⌝ → traversal_inv Σ Hg1 Hg2 Hg3 γ_m t0 j k (ps0 !!! j) (ss0 !!! j)) }}}
+        traverse_rec #k #preds #succs #i @ ⊤
+      {{{ (ps ss: list Node) (res: bool), 
+            RET (#preds, #succs, #res);
+            is_array Σ Hg1 preds ps ∗ is_array Σ Hg1 succs ss
+          ∗ ⌜length ps = L⌝ ∗ ⌜length ss = L⌝
+          ∗ ⌜ps !!! (L-1) = hd⌝ ∗ ⌜ss !!! (L-1) = tl⌝
+          ∗ (∀ i, ⌜i < L⌝ → traversal_inv Σ Hg1 Hg2 Hg3 γ_m t0 i k (ps !!! i) (ss !!! i))
+          ∗ (let c := ss !!! 0 in 
+                ∃ s, past_state Σ Hg1 Hg2 Hg3 γ_m t0 s ∗
+                    ⌜if res then 
+                      k ∈ abs s ∧ k = Key s c ∧ c ∈ FP s ∧ Marki s c 0 = false
+                    else 
+                      k ∉ abs s ∧ k < Key s c ∧ c ∈ FP s⌝) }}}.
+  
+  Lemma traverse_spec (Σ : gFunctors) (H' : heapGS Σ) (H'' : dsG Σ) (H''' : hsG Σ)
+    N γ_t γ_r γ_m γ_mt γ_msy r tid t0 k (hd tl: Node):
+    main_inv Σ H' H'' H''' N γ_t γ_r γ_m γ_mt γ_msy r -∗
+    thread_start Σ H' H'' H''' γ_t γ_mt tid t0 -∗
+    □ update_helping_protocol Σ H' H'' H''' N γ_t γ_r γ_mt γ_msy -∗ 
+    ⌜1 < L ∧ 0 < k < W⌝ -∗
+      {{{ True }}}
+          traverse #hd #tl #k @ ⊤
+      {{{ (preds succs: loc) (ps ss: list Node) (res: bool), 
+            RET (#preds, #succs, #res);
+            (preds ↦∗ ((fun n => # (LitLoc n)) <$> ps))
+          ∗ (succs ↦∗ ((fun n => # (LitLoc n)) <$> ss))
+          ∗ ⌜length ps = L⌝ ∗ ⌜length ss = L⌝
+          ∗ ⌜ps !!! (L-1) = hd⌝ ∗ ⌜ss !!! (L-1) = tl⌝
+          ∗ (∀ i, ⌜i < L⌝ → traversal_inv Σ H' H'' H''' γ_m t0 i k (ps !!! i) (ss !!! i))
+          ∗ (let c := ss !!! 0 in 
+                ∃ s, past_state Σ H' H'' H''' γ_m t0 s ∗
+                    ⌜if res then 
+                      k ∈ abs s ∧ k = Key s c ∧ c ∈ FP s ∧ Marki s c 0 = false
+                    else 
+                      k ∉ abs s ∧ k < Key s c ∧ c ∈ FP s⌝) }}}.
+  Proof.
+    iIntros "#HInv #Thd_st #Upd [%HL %Range_k]". iIntros (Φ) "!# _ Hpost".
+    wp_lam. wp_pures. wp_bind (AllocN _ _)%E. 
+    iApply array_repeat. iPureIntro; lia.
+    iNext. iIntros (preds) "Hpreds".
+    wp_pures. wp_bind (AllocN _ _)%E.
+    iApply array_repeat. iPureIntro; lia.
+    iNext. iIntros (succs) "Hsuccs". wp_pures. iApply fupd_wp.
+    iInv "HInv" as (M0 T0 s0) "(>Ds & >%Habs0 & >Hist & Help & >Templ)".
+    iDestruct "Templ" as (hd' tl')"(HR & SShot0 & Res & %PT0 & %Trans_M0)".
+    iAssert (⌜hd' = hd ∧ tl' = tl⌝)%I as %[-> ->]. admit.
+    iAssert (⌜per_tick_inv hd tl s0⌝)%I as %PT_s0.
+    { iApply (per_tick_current with "[%] [%] [$Hist]"); try done. }
+    iPoseProof (traversal_inv_hd_tl with "[%] [%] [%] [%] [#] [Hist]") 
+      as ">(#HtrL & Hist)"; try done.
+    iModIntro. iSplitR "Hpreds Hsuccs Hpost".
+    { iNext. iExists M0, T0, s0. iFrame "∗%". iExists hd, tl. iFrame "∗%". }
+    iModIntro.      
+    wp_apply (traverse_rec_spec with "[] [] [] [] [Hpreds Hsuccs]"); try done.
+    iFrame "Hpreds Hsuccs".
+    iSplitR. iPureIntro. by rewrite replicate_length.
+    iSplitR. iPureIntro. by rewrite replicate_length.
+    iSplitR. iPureIntro. clear -HL; lia.
+    iSplitR. iPureIntro. rewrite lookup_total_replicate_2. done. lia.
+    iSplitR. iPureIntro. rewrite lookup_total_replicate_2. done. lia.
+    iIntros (j) "%Hj". 
+    assert (j = L-1) as -> by lia. rewrite !lookup_total_replicate_2.
+    all : try lia. iFrame "HtrL".
+  Admitted.  
+
+End TRAVERSE_SPEC.
+
+Declare Module TR_SPEC : TRAVERSE_SPEC.
+Export TR_SPEC.
